<subsection xmlns:xi="http://www.w3.org/2001/XInclude" xml:id="subsec-equation-of-a-circle">
<title>Equation of a Circle</title>
<p>We now construct an equation that the coordinates (<em>x</em>,<em>y</em>) of the points on the circle should satisfy. So, let P(<em>x,y</em>) be any point on a circle of radius <em>r</em> and center C(<em>h,k</em>) (see, Figure 4.7). Then, the definition of a circle requires that</p>
<p><alert>|</alert>CP<alert>|</alert> = <em>r</em></p>
<p>⇒</p>
<p>or</p>
<table>
<tabular>
<row>
<cell><image source="/media/png72/imageC2254.png" /></cell>
<cell><p>(Standard equation of a circle with</p>
<p>center (<em>h</em>,k) and radius <em>r.</em></p></cell>
</row>
</tabular>
</table>
<p>In particular, if the center is at origin, i.e., (<em>h,k</em>) = (0,0), the equation is</p>
<table>
<tabular>
<row>
<cell><image source="/media/png72/imageC2255.png" /></cell>
<cell>(Standard Equation of a circle of radius <em>r</em> centered at origin)</cell>
</row>
</tabular>
</table>
<p><alert>Example 4.8</alert>: Find an equation of the circle with radius 4 and center (−2, 1).</p>
<p><alert>Solution</alert>: Using the standard equation of a circle in which the center (<em>h, k</em>) <em>=</em> (−2, 1) and radius <em>r =</em> 4 we obtain the equation</p>
<p><image source="/media/png72/imageC2256.png" />.</p>
<p><alert>Example 4.9</alert>: Find the equation of a circle with endpoints of a diameter at P(–2, 0) and Q(4, 2).</p>
<p><alert>Solution</alert>: The center of the circle C(<em>h,k</em>) is the mid-point of the diameter. Hence, <image source="/media/png72/imageC2257.png" />. Also, for its radius <em>r</em>, <em>r</em><sup>2</sup> = <alert>|</alert>CP<alert>|</alert><sup>2</sup>=(1+2)<sup>2</sup>+(1 – 0)<sup>2</sup>=10.</p>
<p>Thus, the equation of the circle is (<em>x – h</em>)<sup>2</sup>+(<em>y –k</em>)<sup>2</sup> <em>=</em> <em>r</em><sup>2</sup> . That is,</p>
<p>(<em>x –</em> 1)<sup>2</sup>+(<em>y –</em>1)<sup>2</sup> <em>=</em> 10 .</p>
<p><alert>Example 4.10</alert>: Suppose P(−2,4) and Q(5,3) are points on a circle whose center is on <em>x</em>-axis. Find the equation of the circle.</p>
<p><alert>Solution</alert>: We need to obtain the center C and radius <em>r</em> of the circle to construct its equation. As the center is on <em>x</em>-axis, its second coordinate is 0. Therefore, let C(<em>h</em>,0) be the center of the circle. Note that |PC|<sup>2</sup> = |QC|<sup>2</sup> = <em>r</em><sup>2</sup> as both P and Q are on the circle. So, from the first equality we get (−2−<em>h</em>)<sup>2</sup> + 4<sup>2</sup> = (5−<em>h</em>)<sup>2</sup> + 3<sup>2</sup> . Solving this for <em>h</em> we get <em>h=</em>1. Hence, the center is at C(1, 0) and <em>r</em><sup>2</sup> = |QC|<sup>2</sup> = (5−1)<sup>2</sup> + 3<sup>2</sup> =25. Therefore, the equation of the circle is</p>
<p>(<em>x</em>−1)<sup>2</sup> + <em>y</em><sup>2</sup> =25.</p>
<p><alert>Example 4.11:</alert> Determine whether the given equation represents a circle. If it does, identify its center and radius and sketch its graph.</p>
<p>(a) <image source="/media/png72/imageC2258.png" /></p>
<p>(b) <em>x</em><sup>2</sup> + <em>y</em><sup>2</sup> + 2<em>x</em> − 6<em>y</em> +10 = 0</p>
<p>(c) <em>x</em><sup>2</sup> + <em>y</em><sup>2</sup> + 2<em>x</em> − 6<em>y</em> + 11 = 0</p>
<p><alert>Solution</alert>: We need to rewrite each equation in standard form to identify its center and radius. We do this by completing the square on the x-terms and y-terms of the equation as follows:</p>
<p>(a) <image source="/media/png72/imageC2259.png" /> (Grouping x-terms and y-terms)</p>
<p>⇔ <image source="/media/png72/imageC2260.png" /> (Adding 1<sup>2</sup> and 3<sup>2</sup> to both sides)</p>
<p>⇔ ( <em>x</em> + 1)<sup>2</sup> + (<em>y</em> – 3)<sup>2</sup> = 3.</p>
<p>Comparing this with the standard equation of circle this is equation of a circle with center (<em>h</em>, <em>k</em>) = (–1, 3) and radius <image source="/media/png72/imageC2261.png" />. The graph of the circle is sketched in Figure 4.8</p>
<p>(b) Following the same steps as in (a), you can see that <em>x</em><sup>2</sup> + <em>y</em><sup>2</sup> + 2<em>x</em> − 6<em>y</em> +10 = 0 is equivalent to ( <em>x</em> + 1)<sup>2</sup> + (<em>y</em> – 3)<sup>2</sup> = 0.</p>
<p>This is satisfied by the point (−1, 3) only. The locus of this equation is considered as a point-circle, circle of zero radius (sometimes called degenerated circle).</p>
<p>(c) Again following the same steps as in (a), you can see that <em>x</em><sup>2</sup> + <em>y</em><sup>2</sup> + 2<em>x</em> − 6<em>y</em> +11 = 0 is equivalent to ( <em>x</em> + 1)<sup>2</sup> + (<em>y</em> – 3)<sup>2</sup> = −1.</p>
<p>Note that this does not represent a circle; in fact it has no locus at all (Why? ).</p>
<table>
<tabular>
<row>
<cell><p><alert>Remark:</alert> Consider an equation of the form</p>
<p><em>x</em><sup>2</sup> + <em>y</em><sup>2</sup> + D<em>x</em> + E<em>y</em> + F = 0.</p>
<p>By completing the square you can show the following:</p>
<ul>
<li>
<p>If D<sup>2</sup> + E<sup>2</sup> − 4F &gt; 0 , then the equation represents a circle with</p>
</li>
</ul>

<p>center <image source="/media/png72/imageC2262.png" /> and radius <image source="/media/png72/imageC2263.png" />.</p>

<ul>
<li>
<p>If D<sup>2</sup> + E<sup>2</sup> − 4F = 0 , then the equation is satisfied by the point <image source="/media/png72/imageC2262.png" /> only. In this case the locus of the equation is called <alert>point-circle</alert> (circle of zero radius).</p>
</li>
<li>
<p>If D<sup>2</sup> + E<sup>2</sup> − 4F &lt; 0 , then the equation has no locus.</p>
</li>
</ul></cell>
</row>
</tabular>
</table>
<p><alert>Exercise 4.2.2</alert></p>
<table>
<tabular>
<row header="yes">
<cell><p>1. Determine whether each of the following points is inside, outside or on the circle with equation <image source="/media/png72/imageC2264.png" />.</p>
<p>(a) (−1, 2), (b) (3/2, 2) (c) <image source="/media/png72/imageC2265.png" /> (d) (−1, 3/2 )</p>
<p>2. Find an equation of the circle whose endpoints of a diameter are (0, −3) and (3, 3).</p>
<p>3. Determine an equation of a circle whose center is on <em>y</em>-axis and radius is 2.</p>
<p>4. Find an equation of the circle passing through (1, 0) and (0, 1) which has its center on the line 2<em>x</em> + 2<em>y</em> =5.</p>
<p>5. Find the value(s) of <em>k</em> for which the equation 2<em>x</em><sup>2</sup> + 2<em>y</em><sup>2</sup> <em>+</em> 6<em>x –</em> 4<em>y + k =</em> 0 represent a circle.</p>
<p>6. An equation of a circle is <image source="/media/png72/imageC2266.png" />. If the radius of the circle is 2, .then what is the coordinates of its center?</p>
<p>7. Find equation of the circle passing through (0,0), (4, 0) and (2, 2).</p>
<p>8. Find equation of the circle inscribed in the triangle with vertices (−7, −10), (−7, 15), and (5,−1).</p>
<p>9. In each of the following, check whether or not the given equation represents a circle. If the equation represents a circle, then identify its center and the length of its diameter.</p>
<p>(a) <image source="/media/png72/imageC2267.png" /> (d) <image source="/media/png72/imageC2268.png" /></p>
<p>(b) <image source="/media/png72/imageC2269.png" /> (e) <image source="/media/png72/imageC2270.png" /></p>
<p>(c) <image source="/media/png72/imageC2271.png" /> (f) <image source="/media/png72/imageC2272.png" /></p></cell>
</row>

<row>
<cell>10. Show that <em>x</em><sup>2</sup> + <em>y</em><sup>2</sup> + D<em>x</em> + E<em>y</em> + F = 0 represents a circle of positive radius iff D<sup>2</sup> + E<sup>2</sup> − 4F &gt; 0.</cell>
</row>
</tabular>
</table>
</subsection>
