<subsection xmlns:xi="http://www.w3.org/2001/XInclude" xml:id="subsec-argument-amplitude-of-a-complex">
<title>Argument (Amplitude) of a complex number</title>
<definition xml:id="def-argument-amplitude-of-a-complex">
    <statement>
        <p>
            Argument of a complex number <m>z = x+iy</m> is the angle formed by the complex number <m>z = x+iy</m> with the positive x-axis. The argument of a complex number <m>z = x+iy</m> is deonted by <m>\textbf{argz}</m> and is given by arg(z) = <m>\text{tan}^{- 1}(\frac{y}{x})\text{.}</m>
        </p>
        <p>
            The particular argument of <m>z</m> that lies in the range <m>- \pi &lt; \theta \leq \pi</m> is called the principal argument of <m>z</m> and is dented by Argz.
        </p>
    </statement>
</definition>
<p>
    Notes : <m>i) Argz \ \ \in \left ( -\pi , \pi \right ]</m>.
</p>
<p>
    <m> \ \ \ \ \ \ \ \ \ \ \ \ ii) \text{If} \ 0 \leq \ \text{Argz} \ \leq \pi,</m> move counter clock wise direction, if not move the other direction.
</p>
<example>
    <statement>
        <p>
            Find the argument of the following complex numbers:
        </p>
        <p>
            <ol marker="a)">
                <li>
                    <p>
                        <m>z = 1 + i</m>
                    </p>
                </li>
                <li>
                    <p>
                        <m>z = - 2 + 2 \sqrt{3i}</m>
                    </p>
                </li>
                <li>
                    <p>
                        <m>z = - \sqrt{3} - i</m>
                    </p>
                </li>
            </ol>
        </p>
    </statement>
    <solution>
        <p>
            <m>a) \ \ z = 1 + i</m>
        </p>
        <p>
            <m>\text{Arg}z = \text{tan}^{- 1}\left(\frac{1}{1}\right) = \text{tan}^{- 1}\left(1 \right) = \frac{\pi}{4}</m>
        </p>
        <p>
            <m>b) \ \ z = - 2 + 2 \sqrt{3}i</m>
        </p>
        <p>
            <m>\text{Arg}z = \text{tan}^{- 1}\left(\frac{2 \sqrt{3}}{-2}\right) = \text{tan}^{- 1}(-\sqrt{3}) = \frac{2 \pi}{3}</m>
        </p>
        <p>
            <m>c) \ \ z = - \sqrt{3} - i</m>
        </p>
        <p>
            <m>\text{Arg}z = \text{tan}^{- 1}\left(\frac{-1}{-\sqrt{3}}\right) = \text{tan}^{- 1}\left(\frac{1}{\sqrt{3}}\right) = \frac{-5 \pi}{6}</m>
        </p>
    </solution>
</example>

<p>
    <me>
        \textbf{Properties of Arguments}
    </me>
</p>
<p>
    <m>i) \ \ \text{Arg}(z_{1} \cdot z_{2}) = \text{Arg}z_{1} \ + \ \text{Arg}z_{2}</m>
</p>
<p>
    <m>ii) \ \ \text{Arg}\left(\frac{z_{1}}{z_{2}}\right) = \text{Arg}z_{1} \ - \ \text{arg}z_{2}</m>
</p>

<example>
    <statement>
        <p>
            Find the principal argument of <m>\ a)\ (1 + i)\ ( - 1 - i)\ \ \ \ b)\ (\frac{- 2 + 2i}{1 - i})</m>
        </p>
    </statement>
    <solution>
        <p>
            <m>a) \ \ \text{Arg} \ (1 + i)(-1 - i) = \text{Arg} \ (1 + i) + \text{Arg} \ (-1 - i) = \frac{\pi}{4} + (\frac{-3 \pi}{4}) = \underline{\underline{\frac{-\pi}{2}}} </m>
        </p>
        <p>
            <m>b) \ \ \text{Arg} \left(\frac{- 2 + 2i}{1 - i}\right) = \text{Arg}(-2 + 2i) - \text{Arg}(1 - i) = (\frac{3 \pi}{4}) - (-\frac{\pi}{4}) = \frac{4 \pi}{4} = \underline{\underline{\pi}}</m>
        </p>
    </solution>
</example>

<exercise><stack source="/questions/top/Mathematics-for-NS-&amp;-SS-23-24-Question-Bank/The-Real-and-Complex-Number-Systems-(NS)/Argument-(amplitude)-of-a-complex-number/Modulus-and-Argument-of-a-Complex-Number.xml" /></exercise>
<exercise><stack source="/questions/top/Mathematics-for-NS-&amp;-SS-23-24-Question-Bank/The-Real-and-Complex-Number-Systems-(NS)/Argument-(amplitude)-of-a-complex-number/Modulus-and-Argument-of-Complex-Numbers-and-Their-Conjugates.xml" /></exercise>
</subsection>

