<subsection xmlns:xi="http://www.w3.org/2001/XInclude" xml:id="subsec-polar-form-of-a-complex">
<title> Polar form of a complex number</title>
<definition xml:id="def-polar-form-of-a-complex">
    <statement>
        <p>
            Let <m>r</m> and <m>\theta</m> be polar coordinates of the point (x, y) of the complex number <m>z = x+iy</m>. Since x = <m>r\text{cos}\theta</m>and y = <m>r\text{sin}\theta</m>, then the complex number can be written as : <m>\underline{\underline{\ z = r(\text{cos}\theta + i\text{sin}\theta)}}</m> which is called polar form, where <m>r</m> is modulus of <m>z</m> and <m>\ \theta\ </m>is principal argument of <m>z</m>.
        </p>
    </statement>
</definition>

<example>
    <statement>
        <p>
            Express the following complex numbers in polar form:
        </p>
        <p>
            <m>a)\ z = 1 + i </m>
        </p>
        <p>
            <m>\text{solution}:\ r = \sqrt{2}\ \text{and}\ \theta = \text{tan}^{- 1}(1) = \frac{\pi}{4} \text{.}</m>
        </p>
        <p>
            <m>\ \text{Thus},\ z = \sqrt{2}(\text{cos} \frac{\pi}{4} + i\text{sin} \frac{\pi}{4})\text{.}</m>
        </p>
        <p>
            <m>b)\ z = 3 - 3i\ \text{solution}:\ r = \sqrt{18}\ \text{and}\ \theta = \text{tan}^{- 1}( - 1) = - \frac{\pi}{4}\text{.}</m>
        </p>
        <p>
            <m>\text{solution}: \ r = \sqrt{\text{18}}\ \text{and}\ \theta = \text{tan}^{- 1}( - 1) = - \pi 4\text{.}\  \\</m>
        </p>
        <p>
            <m>\text{Thus},\ z = \sqrt{\text{18}}(\text{cos} - \frac{\pi}{4} + i\text{sin} - \frac{\pi}{4}) = \sqrt{\text{18}}(\text{cos}\frac{\pi}{4} - i\text{sin}\frac{\pi}{4})\text{.} \\</m>
        </p>
    </statement>
</example>

<p>
    <me>\textbf{Multiplication and division in polar forms}</me>
</p>
<p>
    <m>\text{If} \ z_{1}\ = r_{1}(\text{cos}\theta_{1} + i\text{sin}\theta_{1}) \ \ \ \text{and} \ \ \ \ z_{2} = r_{2}(\text{cos}\theta_{2} + i\text{sin}\theta_{2}), \text{then}</m>
</p>
<p>
    <m>a) \ \ z_{1} \cdot z_{2} = r_{1} \cdot r_{2}(\text{cos}(\theta_{1} + \theta_{2}) + i\text{sin}(\theta_{1} + \theta_{2}))</m>
</p>
<p>
    <m>b) \ \ \frac{z_{1}}{z_{2}} = \frac{r_{1}} {r_{2}}(\text{cos}(\theta_{1} - \theta_{2}) + i\text{sin}(\theta_{1} - \theta_{2}))</m>.
</p>
<p>
    <m>\textbf{Proof:}</m>
</p>
<p>
    <m>z_{1} \cdot z_{2} = r_{1}(\text{cos}\theta_{1} + i\text{sin}\theta_{1}) \cdot r_{2}(\text{cos}\theta_{2} + i\text{sin}\theta_{2})</m>
</p>
<p>
    <m> \ \ \ \ \ \ \ \ \ \ \ = r_{1} \cdot r_{2} \left [ \text{cos}\theta_{1}(\text{cos}\theta_{2} + i\text{sin}\theta_{2}) + i\text{sin}\theta_{1}(\text{cos}\theta_{2} + i\text{sin}\theta_{2}) \right ]</m>
</p>
<p>
    <m> \ \ \ \ \ \ \ \ \ \ \ = r_{1} \cdot r_{2} \left [ \text{cos}\theta_{1}\text{cos}\theta_{2} + i\text{cos}\theta_{1}\text{sin}\theta_{2} + i\text{sin}\theta_{1}\text{cos}\theta_{2} - \text{sin}\theta_{1}\text{sin}\theta_{2} \right ]</m>
</p>
<p>
    <m> \ \ \ \ \ \ \ \ \ \ \ = r_{1} \cdot r_{2} \left [ \text{cos}\theta_{1}\text{cos}\theta_{2} - \text{sin}\theta_{1}\text{sin}\theta_{2} + i(\text{cos}\theta_{1}\text{sin}\theta_{2} + \text{sin}\theta_{1}\text{cos}\theta_{2}) \right ]</m>
</p>
<p>
    <m> \ \ \ \ \ \ \ \ \ \ \ = \underline{\underline{ r_{1} \cdot r_{2} \left [ \text{cos}(\theta_{1} + \theta_{2}) + i \ \text{sin}(\theta_{1} + \theta_{2})\right ]}}</m>
</p>
<p>
    <m>\text{Thus,} \ z_{1} \cdot z_{2} = r_{1} \cdot r_{2}(\text{cos}(\theta_{1} + \theta_{2}) + i \ \text{sin}(\theta_{1} + \theta_{2}))</m>
</p>

<p><alert>Example 2.53:</alert> <m>\ \text{If}\ z_{1} = 6\ (\text{cos}\pi 2\  + i\text{sin}\pi 2)\ \text{and}\ z_{2} = 2\ (\text{cos}\pi 3\  + i\text{sin}\pi 3),\ \text{then}\ \text{find}\ </m></p>
<p><m></m> <m>\ a)\ z\ _{1}\text{.}\ z_{2}\ b)\ \frac{z_{1}}{z_{2}}</m></p>
<ul>
<li><p><alert>Argument of a product</alert></p></li>
</ul>
<table>
<tabular>
<row>
<cell>The argument of the product of two complex numbers is the sum of their arguments.</cell>
</row>
</tabular>
</table>
<p><image source="/./media/image42.png" style="width:4.91319in;height:2.38542in" /></p>
<p><alert>Proof:</alert></p>

<p><m></m> <alert>Argument of a quotient</alert></p>

<table>
<tabular>
<row>
<cell>The argument of the quotient of two complex numbers is the difference of their arguments.</cell>
</row>
</tabular>
</table>
<p><alert>Proof:</alert></p>
<p><alert>Example 2.54:</alert> <m>\text{arg}(\frac{- 4}{1 + \sqrt{3}\ i}) = \text{arg}( - 4) - \text{arg}(\ 1 + \sqrt{3}\ i) = \pi - \pi 3 = \ 2\pi 3</m></p>
<table>
<tabular>
<row>
<cell><alert>De Moivre’s Formula</alert></cell>
</row>
</tabular>
</table>
<p><alert>Example 2.55:</alert> Express<m>\ (2 + 2i)^{\text{100}}</m> in polar form.</p>
<p><alert>Example 2.56:</alert> Express<m>(\sqrt{3} + i)^{\text{60}}\ </m> in polar form.</p>
<table>
<tabular>
<row>
<cell><p><alert>Euler’s formula</alert></p>
<p>The complex number <m>z = r(\text{cos}\theta + i\text{sin}\theta)</m> can be written in exponential form as: <m>z = \text{re}^{\text{iθ}}</m> which is called Euler’s formula.</p></cell>
</row>
</tabular>
</table>
<p><alert>Example 2.57</alert>: Express the complex number z = 1+i using Euler’s formula.</p>
<p><m>\begin{matrix}
\text{Solution}:\ z = 1 + i \\
\text{Now}\ r = \sqrt{2}\  \land \ \theta = \pi 4\  \Rightarrow \ z = \text{re}^{\text{iθ}} = \underline{\underline{\sqrt{2}e^{\pi\ i4}}} \\
\end{matrix}</m></p>
<p><alert>Example 2.58</alert>: Express the complex number <m>z = 1 + \sqrt{3}\ i\ </m> using Euler’s formula.</p>
<p><alert>Example 2.59</alert>: Express the complex number <m>z = (\sqrt{3}\  + i\ )^{7}</m> using Euler’s formula.</p>

<exercise><stack source="/questions/top/Mathematics-for-NS-&amp;-SS-23-24-Question-Bank/The-Real-and-Complex-Number-Systems-(NS)/Polar-form-of-a-complex-number/Converting-Complex-Numbers-Rectangular-to-Polar-Form.xml" /></exercise>
<exercise><stack source="/questions/top/Mathematics-for-NS-&amp;-SS-23-24-Question-Bank/The-Real-and-Complex-Number-Systems-(NS)/Polar-form-of-a-complex-number/Conversion-to-Polar-Form-Complex-Number-z-=-x-+-yi.xml" /></exercise>
</subsection>

