<subsection xmlns:xi="http://www.w3.org/2001/XInclude" xml:id="subsec-conjugate-of-a-complex-number">
<title>Conjugate of a complex number</title>
<definition xml:id="def-">
    <statement>
        <p>
            The conjugate of a complex number z = x+iy is denoted by <m>\ \overline{z}</m> and is defined as <m>\ \overline{z}</m> = x-iy. It can be represented by the point (x, -y) which is the reflection of the point (x, y) about the x-axis.
        </p>
    </statement>
</definition>

<image source="/./media/image40.png" width="60%" />

<example>
    <statement>
        <p>
            Find the conjugate of the complex number <m>z = 2+9i</m>.
        </p>
    </statement>
    <solution>
        <p>
            <m>\ \ \ \ \ \ z = 2+9i</m>
        </p>
        <p>
            <m> \Rightarrow \overline{z} = 2-9i</m>.
        </p>
    </solution>
</example>

<p>
    <me>
        \textbf{Properties of Conjugate}
    </me>
</p>
<p>
    <m> a. \overline{\overline{z}} = z</m>
</p>
<p>
    <m> b. z + \overline{z} = 2x =2Re{(z)} = 2  \left (\frac{z + \overline{z}}{2} \right )</m>
</p>
<p>
    <m> c. z - \overline{z} = 2iy = 2Im{(z)}</m>
</p>
<p>
    <m> d. \overline{z_1 + z_2} = \overline{z_1} + \overline{z_2}</m>
</p>
<p>
    <m> e. \overline{z_1 - z_2} = \overline{z_1} - \overline{z_2}</m>
</p>
<p>
    <m> f. \overline{z_1 \cdot z_2} = \overline{z_1} \cdot \overline{z_2}</m>
</p>
<p>
    <m> g. \overline{({\frac{z_1}{z_2}})} = \frac{\overline{z_1}}{\overline{z_2}}</m>
</p>
<p>
    
</p>
<p>
    proof : a) let <m>z = x + iy</m>
</p>
<p>
    <m>\ \ \ \ \ \ \ \ \ \ \ \ \ \ \ \Rightarrow \overline{z} = x - iy</m>
</p>
<p>
    <m>\ \ \ \ \ \ \ \ \ \ \ \ \ \ \  \Rightarrow \overline{\overline{z}} = x + iy = z</m>
</p>
<p>
    <m>\ \ \ \ \ \ \ \ \ \ \ \ \ \ \  \ \therefore \ \overline{\overline{z}} = z</m>.
</p>
<p>
    <m> \ \ \ \ \ \ \ \ \ \ \ \ \ d) \ \text{Let} \ z_{1} = x_{1} + iy_{1} </m> &amp; <m> z_{2} = x_{2} + iy_{2}</m>
</p>
<p>
    <m>\ \ \ \ \ \ \ \ \ \ \ \ \ \ \  \ \Rightarrow \overline{z_{1}} = x_{1} - iy_{1} \ \ \ </m> &amp; <m> \ \ z_{2} = x_{2} - iy_{2}</m>
</p>
<p>
    Now <m> \overline{z_1 + z_2} = \overline{(x_{1} + iy_{1}) + (x_{2} + iy_{2})} = \overline{(x_{1} + x_{2}) + i(y_{1} + y_{2})} = (x_{1} + x_{2}) + i(y_{1} + y_{2})</m>
</p>
<p>
    <m>\ \ \ \ \ \ \ \ \ \ \ \ \ \ \ \ \ \ \ \ \ \ \ \ \ \ \ \ \ \ \ \ \ \ \ \ \ \ \ \ \ \ \ \ \ \ \ \ \ \ \ \ \ \ \ \ \ \ \ \ \ \ \ \ \ \ \ \ \ \ \ \ \ \ \ \ \ \  \ \ \ \ \ \ \ \ \ \ \ \ \ \ \ \ \ \ \ \ \ \ \ \ \ \ \ \ \ \ \ \ \ \ \ \ \ \ = x_{1} - iy_{1} + x_{2} - iy_{2}</m>
</p>
<p>
    <m>\ \ \ \ \ \ \ \ \ \ \ \ \ \ \ \ \ \ \ \ \ \ \ \ \ \ \ \ \ \ \ \ \ \ \ \ \ \ \ \ \ \ \ \ \ \ \ \ \ \ \ \ \ \ \ \ \ \ \ \ \ \ \ \ \ \ \ \ \ \ \ \ \ \ \ \ \ \ \ \ \ \ \ \ \ \ \ \ \ \ \ \ \ \ \ \ \ \ \ \ \ \ \ \ \ \ \ \ \ \ \ \ \ \ \ \ = \overline{z_1} + \overline{z_2}</m>
</p>
<p>
    The others are left for the reader.
</p>
</subsection>
