<subsection xmlns:xi="http://www.w3.org/2001/XInclude" xml:id="subsec-compound-(or-complex)-propositions">
<title>Compound (or complex) propositions</title>
<p>So far, what we have done is simply to define the logical connectives, and express them through algebraic symbols. Now we shall learn how to form propositions involving more than one connective, and how to determine the truth values of such propositions.</p>
<table>
<tabular>
<row>
<cell><alert>Definition 1.2:</alert> The proposition formed by joining two or more proposition by connective(s) is called a compound statement.</cell>
</row>
</tabular>
</table>
<p><alert>Note:</alert> We must be careful to insert the brackets in proper places, just as we do in arithmetic. For example, the expression <m>p \Longrightarrow q \land r</m> will be meaningless unless we know which connective should apply first. It could mean <m>(p \Longrightarrow q) \land r</m> or <m>p \Longrightarrow (q \land r)</m>, which are very different propositions. The truth value of such complicated propositions is determined by systematic applications of the rules for the connectives.</p>
<table>
<tabular>
<row>
<cell>The possible truth values of a proposition are often listed in a table, called a <alert>truth table</alert>. If <m>p</m> and <m>q</m> are propositions, then there are four possible combinations of truth values for <m>p</m> and <m>q</m>. That is, <m>\text{TT}</m>, <m>\text{TF}</m>, <m>\text{FT}</m> and <m>\text{FF}</m>. If a third proposition <m>r</m> is involved, then there are eight possible combinations of truth values for <m>p</m>,<m>q</m> and <m>r</m>. In general, a truth table involving “<m>n</m>” propositions <m>p_{1}</m>,<m>\ p_{2}</m>,…,<m>\ p_{n}</m> contains <m>2^{n}</m> possible combinations of truth values. So, we use truth tables to determine the truth value of a compound proposition based on the truth value of its constituent component propositions.</cell>
</row>
</tabular>
</table>
<p><alert>Examples 1.6:</alert></p>
<ol type="a">
<li><p>Suppose <m>p</m> and <m>r</m> are true and <m>q</m> and <m>s</m> are false.</p></li>
</ol>
<p>What is the truth value of <m>\left( p \land q \right) \Longrightarrow (r \vee s)</m>?</p>
<ol type="i">
<li>
<p>Since <m>p</m> is true and <m>q</m> is false, <m>p \land q</m> is false.</p>
</li>
<li>
<p>Since <m>r</m> is true and <m>s</m> is false, <m>r \vee s</m> is true.</p>
</li>
<li>
<p>Thus by applying the rule of implication, we get that <m>\left( p \land q \right) \Longrightarrow (r \vee s)</m> is true.</p>
</li>
</ol>
<ol start="2" type="a">
<li><p>Suppose that a compound proposition is symbolized by</p></li>
</ol>
<p><me>(p \vee q) \Longrightarrow (r\mathbf{\Longleftrightarrow}\neg s)</me></p>
<p>and that the truth values of <m>p,q,r,</m> and <m>s</m> are <m>T,F,F,</m> and <m>T</m>, respectively. Then the truth value of <m>p \vee q</m> is <m>T</m>, that of <m>\neg s</m> is <m>F</m>, that of <m>r\mathbf{\Longleftrightarrow}\neg s</m> is <m>T</m>. So the truth value of <m>(p \vee q) \Longrightarrow (r\mathbf{\Longleftrightarrow}\neg s)</m> is <m>T</m>.</p>
<p><alert>Remark:</alert> When dealing with compound propositions, we shall adopt the following convention on the use of parenthesis. Whenever “<image source="/media/imageA8.png" />” or “<image source="/media/imageA9.png" />” occur with “<image source="/media/imageA10.png" />” or “<image source="/media/imageA11.png" />”, we shall assume that “<image source="/media/imageA8.png" />” or “<image source="/media/imageA9.png" />” is applied first, and then “<image source="/media/imageA10.png" />” or “<image source="/media/imageA11.png" />” is then applied. For example,</p>
<p><m>p \land q \Longrightarrow r</m> means <m>(p \land q) \Longrightarrow r</m></p>
<p><m>p \vee q\mathbf{\Longleftrightarrow}r</m> means <m>(p \vee q)\mathbf{\Longleftrightarrow}r</m></p>
<p><m>\neg q \Longrightarrow \neg p</m> means <m>\left( \neg q \right) \Longrightarrow (\neg p)</m></p>
<p><m>\neg q \Longrightarrow p\mathbf{\Longleftrightarrow}r</m> means <m>((\neg q) \Longrightarrow p)\mathbf{\Longleftrightarrow}r</m></p>
<p>However, it is always advisable to use brackets to indicate the order of the desired operations. .</p>
<table>
<tabular>
<row>
<cell><alert>Definition 1.3:</alert> Two compound propositions <m>P</m> and <m>Q</m> are said to be <em><alert>equivalent</alert></em> if they have the same truth value for all possible combinations of truth values for the component propositions occurring in both <m>P</m> and <m>Q</m>. In this case we write <m>P \equiv Q</m>.</cell>
</row>
</tabular>
</table>
<p><alert>Example 1.7:</alert> Let <m>P:p \Longrightarrow q</m>.</p>
<p><m>Q:\neg(p \land \neg q)</m><image source="/media/imageA4.png" /><m>Q:\neg q \Longrightarrow \neg p</m>.</p>
<table>
<tabular>
<row header="yes">
<cell><me>\mathbf{p}</me></cell>
<cell><me>\mathbf{q}</me></cell>
<cell><me>\mathbf{\neg}p</me></cell>
<cell><me>\mathbf{\neg}q</me></cell>
<cell><me>\mathbf{p} \Longrightarrow q</me></cell>
<cell><me>\mathbf{\neg}q \Longrightarrow \neg p</me></cell>
</row>

<row>
<cell><p><me>\mathbf{T}</me></p>
<p><me>\mathbf{T}</me></p>
<p><me>\mathbf{F}</me></p>
<p><me>\mathbf{F}</me></p></cell>
<cell><p><me>\mathbf{T}</me></p>
<p><me>\mathbf{F}</me></p>
<p><me>\mathbf{T}</me></p>
<p><me>\mathbf{F}</me></p></cell>
<cell><p><me>\mathbf{F}</me></p>
<p><me>\mathbf{F}</me></p>
<p><me>\mathbf{T}</me></p>
<p><me>\mathbf{T}</me></p></cell>
<cell><p><me>\mathbf{F}</me></p>
<p><me>\mathbf{T}</me></p>
<p><me>\mathbf{F}</me></p>
<p><me>\mathbf{T}</me></p></cell>
<cell><p><me>\mathbf{T}</me></p>
<p><me>\mathbf{F}</me></p>
<p><me>\mathbf{T}</me></p>
<p><me>\mathbf{T}</me></p></cell>
<cell><p><me>\mathbf{T}</me></p>
<p><me>\mathbf{F}</me></p>
<p><me>\mathbf{T}</me></p>
<p><me>\mathbf{T}</me></p></cell>
</row>
</tabular>
</table>
<p>Then, <m>P</m> is equivalent to <m>Q</m>, since columns 5 and 6 of the above table are identical.</p>
<p><alert>Example 1.8:</alert> Let <m>P:p \Longrightarrow q</m>.</p>
<p><m>Q:\neg p \Longrightarrow \neg q</m>.</p>

<p>Then</p>

<table>
<tabular>
<row header="yes">
<cell><me>\mathbf{p}</me></cell>
<cell><me>\mathbf{q}</me></cell>
<cell><me>\mathbf{\neg}p</me></cell>
<cell><me>\mathbf{\neg}q</me></cell>
<cell><me>\mathbf{p} \Longrightarrow q</me></cell>
<cell><me>\neg\mathbf{p \Longrightarrow}\neg\mathbf{q}</me></cell>
</row>

<row>
<cell><p><me>\mathbf{T}</me></p>
<p><me>\mathbf{T}</me></p>
<p><me>\mathbf{F}</me></p>
<p><me>\mathbf{F}</me></p></cell>
<cell><p><me>\mathbf{T}</me></p>
<p><me>\mathbf{F}</me></p>
<p><me>\mathbf{T}</me></p>
<p><me>\mathbf{F}</me></p></cell>
<cell><p><me>\mathbf{F}</me></p>
<p><me>\mathbf{F}</me></p>
<p><me>\mathbf{T}</me></p>
<p><me>\mathbf{T}</me></p></cell>
<cell><p><me>\mathbf{F}</me></p>
<p><me>\mathbf{T}</me></p>
<p><me>\mathbf{F}</me></p>
<p><me>\mathbf{T}</me></p></cell>
<cell><p><me>\mathbf{T}</me></p>
<p><me>\mathbf{F}</me></p>
<p><me>\mathbf{T}</me></p>
<p><me>\mathbf{T}</me></p></cell>
<cell><p><me>\mathbf{T}</me></p>
<p><me>\mathbf{T}</me></p>
<p><me>\mathbf{F}</me></p>
<p><me>\mathbf{T}</me></p></cell>
</row>
</tabular>
</table>
<p>Looking at columns 5 and 6 of the table we see that they are not identical. Thus <m>P ≢ Q</m>.</p>
<p>It is useful at this point to mention the non-equivalence of certain conditional propositions. Given the conditional <m>p \Longrightarrow q</m>, we give the related conditional propositions:-</p>
<p><m>q \Longrightarrow p</m>: Converse of <m>p \Longrightarrow q</m></p>
<p><m>\neg p \Longrightarrow \neg q</m>: Inverse of <m>p \Longrightarrow q</m></p>
<p><m>\neg q \Longrightarrow \neg p</m>: Contrapositive of <m>p \Longrightarrow q</m></p>
<p>As we observed from example 1.7, the conditional <m>p \Longrightarrow q</m> and its contrapositve <m>\neg q \Longrightarrow \neg p</m> are equivalent. On the other hand, <m>p \Longrightarrow q ≢ q \Longrightarrow p</m> and <m>p \Longrightarrow q ≢ \neg q \Longrightarrow \neg p</m><m>p \Longrightarrow q ≢ \neg p \Longrightarrow \neg q</m> .</p>
<p><alert>Do not confuse the contrapositive and the converse of the conditional proposition. Here is the difference:</alert></p>
<p><alert>Converse:</alert> The hypothesis of a converse statement is the conclusion of the conditional statement and the conclusion of the converse statement is the hypothesis of the conditional statement.</p>
<p><alert>Contrapositive:</alert> The hypothesis of a contrapositive statement is the negation of conclusion of the conditional statement and the conclusion of the contrapositive statement is the negation of hypothesis of the conditional statement.</p>
<p><alert>Example 1.9:</alert></p>
<ol type="a">
<li><p>If Kidist lives in Addis Ababa, then she lives in Ethiopia.</p></li>
</ol>
<p><alert>Converse:</alert> If Kidist lives in Ethiopia, then she lives in Addis Ababa.</p>

<p><alert>Contrapositive:</alert> If Kidist does not live in Ethiopia, then she does not live in Addis Ababa.</p>

<p><alert>Inverse:</alert> If Kidist does not live in Addis Ababa, then she does not live in Ethiopia.</p>
<ol start="2" type="a">
<li><p>If it is morning, then the sun is in the east.</p></li>
</ol>
<p><alert>Converse:</alert> If the sun is in the east, then it is morning.</p>
<p><alert>Contrapositive:</alert> If the sun is not in the east, then it is not morning.</p>
<p><alert>Inverse:</alert> If it is not morning, then the sun is not the east.</p>
<p>Propositions, under the relation of logical equivalence, satisfy various laws or identities, which are listed below.</p>
<ol type="1">
<li><p>Idempotent Laws</p></li>
</ol>
<ol type="a">
<li><p><m>p \equiv p \vee p</m>.</p></li>
<li><p><m>p \equiv p \land p</m>.</p></li>
</ol>
<ol start="2" type="1">
<li><p>Commutative Laws</p></li>
</ol>
<ol type="a">
<li><p><m>p\  \land \ q \equiv q \land p</m><m>p \land q \equiv q \land p</m> .</p></li>
<li><p><m>p\  \vee \ q \equiv q \vee p</m><m>p \vee q \equiv q \vee p</m> .</p></li>
</ol>
<ol start="3" type="1">
<li><p>Associative Laws</p></li>
</ol>
<ol type="a">
<li><p><m>p \land (q \land r) \equiv (p \land q) \land r</m>.</p></li>
<li><p><m>p \vee (q \vee r) \equiv (p \vee q) \vee r</m>.</p></li>
</ol>
<ol start="4" type="1">
<li><p>Distributive Laws</p></li>
</ol>
<ol type="a">
<li><p><m>p \vee (q \land r) \equiv (p \vee q) \land (p \vee r)</m>.</p></li>
<li><p><m>p \land (q \vee r) \equiv (p \land q) \vee (p \land r)</m>.</p></li>
</ol>
<ol start="5" type="1">
<li><p>De Morgan’s Laws</p></li>
</ol>
<ol type="a">
<li><p><m>\neg(p \land q) \equiv \neg p \vee \neg q</m>.</p></li>
<li><p><m>\neg(p \vee q) \equiv \neg p \land \neg q</m></p></li>
</ol>
<ol start="6" type="1">
<li><p>Law of Contrapositive</p></li>
</ol>
<p><me>p \Longrightarrow q \equiv \neg q \Longrightarrow \neg p</me></p>
<ol start="7" type="1">
<li><p>Complement Law</p></li>
</ol>

<p><m>\neg(\neg p) \equiv p</m>.</p>

</subsection>

