<subsection xmlns:xi="http://www.w3.org/2001/XInclude" xml:id="subsec-tautology-and-contradiction">
<title>Tautology and contradiction</title>
<table>
<tabular>
<row>
<cell><alert>Definition:</alert> A compound proposition is a <alert>tautology</alert> if it is always true regardless of the truth values of its component propositions. If, on the other hand, a compound proposition is always false regardless of its component propositions, we say that such a proposition is a <alert>contradiction</alert>.</cell>
</row>
</tabular>
</table>
<p><alert>Note:</alert> A proposition that is neither a <alert>tautology</alert> nor a <alert>contradiction</alert> is called a <alert>contingency.</alert></p>
<p><alert>Examples 1.10:</alert></p>
<ol type="a">
<li><p>Suppose <m>p</m> is any proposition. Consider the compound propositions <m>p \vee \neg p</m> and <m>p \land \neg p</m>.</p></li>
</ol>
<table>
<tabular>
<row header="yes">
<cell><me>\mathbf{p}</me></cell>
<cell><me>\mathbf{\neg}p</me></cell>
<cell><me>\mathbf{p} \vee \neg p</me></cell>
<cell><me>\mathbf{p} \land \neg p</me></cell>
</row>

<row>
<cell><p><me>\mathbf{T}</me></p>
<p><me>\mathbf{F}</me></p></cell>
<cell><p><me>\mathbf{F}</me></p>
<p><me>\mathbf{T}</me></p></cell>
<cell><p><me>\mathbf{T}</me></p>
<p><me>\mathbf{T}</me></p></cell>
<cell><p><me>\mathbf{F}</me></p>
<p><me>\mathbf{F}</me></p></cell>
</row>
</tabular>
</table>
<p>Observe that <m>p \vee \neg p</m> is a tautology while <m>p \land \neg p</m> is a contradiction.</p>
<ol start="2" type="a">
<li><p>For any propositions <m>p</m> and <m>q</m>. Consider the compound proposition <m>p \Longrightarrow (q \Longrightarrow p)</m>. Let us make a truth table and study the situation.</p></li>
</ol>
<table>
<tabular>
<row header="yes">
<cell><me>\mathbf{p}</me></cell>
<cell><me>\mathbf{q}</me></cell>
<cell><me>\mathbf{q} \Longrightarrow p</me></cell>
<cell><me>\mathbf{p} \Longrightarrow (q \Longrightarrow p)</me></cell>
</row>

<row>
<cell><p><me>\mathbf{T}</me></p>
<p><me>\mathbf{T}</me></p>
<p><me>\mathbf{F}</me></p>
<p><me>\mathbf{F}</me></p></cell>
<cell><p><me>\mathbf{T}</me></p>
<p><me>\mathbf{F}</me></p>
<p><me>\mathbf{T}</me></p>
<p><me>\mathbf{F}</me></p></cell>
<cell><p><me>\mathbf{T}</me></p>
<p><me>\mathbf{T}</me></p>
<p><me>\mathbf{F}</me></p>
<p><me>\mathbf{T}</me></p></cell>
<cell><p><alert>T</alert></p>
<p><alert>T</alert></p>
<p><alert>T</alert></p>
<p><alert>T</alert></p></cell>
</row>
</tabular>
</table>
<p>We have exhibited all the possibilities and we see that for all truth values of the constituent propositions, the proposition <m>p \Longrightarrow (q \Longrightarrow p)</m> is always true. Thus, <m>p \Longrightarrow (q \Longrightarrow p)</m> is a tautology.</p>
<ol start="3" type="a">
<li><p>The truth table for the compound proposition <m>\left( p \Longrightarrow q \right) \Longleftrightarrow (p \land \neg q)</m>.</p></li>
</ol>
<table>
<tabular>
<row header="yes">
<cell><me>\mathbf{p}</me></cell>
<cell><me>\mathbf{q}</me></cell>
<cell><me>\mathbf{\neg}q</me></cell>
<cell><me>\mathbf{p} \land \neg q</me></cell>
<cell><me>\mathbf{p} \Longrightarrow q</me></cell>
<cell><me>\left( p \Longrightarrow q \right) \Longleftrightarrow (p \land \neg q)</me></cell>
</row>

<row>
<cell><p><me>\mathbf{T}</me></p>
<p><me>\mathbf{T}</me></p>
<p><me>\mathbf{F}</me></p>
<p><me>\mathbf{F}</me></p></cell>
<cell><p><me>\mathbf{T}</me></p>
<p><me>\mathbf{F}</me></p>
<p><me>\mathbf{T}</me></p>
<p><me>\mathbf{F}</me></p></cell>
<cell><p><me>\mathbf{F}</me></p>
<p><me>\mathbf{T}</me></p>
<p><me>\mathbf{F}</me></p>
<p><me>\mathbf{T}</me></p></cell>
<cell><p><me>\mathbf{F}</me></p>
<p><me>\mathbf{T}</me></p>
<p><me>\mathbf{F}</me></p>
<p><me>\mathbf{F}</me></p></cell>
<cell><p><me>\mathbf{T}</me></p>
<p><me>\mathbf{F}</me></p>
<p><me>\mathbf{T}</me></p>
<p><me>\mathbf{T}</me></p></cell>
<cell><p><me>\mathbf{F}</me></p>
<p><me>\mathbf{F}</me></p>
<p><me>\mathbf{F}</me></p>
<p><me>\mathbf{F}</me></p></cell>
</row>
</tabular>
</table>
<p>In example 1.10(c), the given compound proposition has a truth value <m>F</m> for every possible combination of assignments of truth values for the component propositions <m>p</m> and <m>q</m>. Thus <m>\left( p \Longrightarrow q \right) \Longleftrightarrow (p \land \neg q)</m> is a contradiction.</p>
<p><alert>Remark:</alert></p>
<ol type="1">
<li><p>In a truth table, if a proposition is a tautology, then every line in its column has <m>T</m> as its entry; if a proposition is a contradiction, every line in its column has <m>F</m> as its entry.</p></li>
<li><p>Two compound propositions <m>P</m> and <m>Q</m> are equivalent if and only if “<m>P\mathbf{\Longleftrightarrow}Q</m>” is a tautology.</p></li>
</ol>
<p><alert>Exercises</alert></p>
<table>
<tabular>
<row header="yes">
<cell><ol type="1">
<li><p>For statements <m>p,q</m> and <m>r</m>, use a truth table to show that each of the following pairs of statements are logically equivalent.</p></li>
</ol>
<ol type="a">
<li><p><m>(p \land q) \Longleftrightarrow p</m> and <m>p \Longrightarrow q</m>.</p></li>
<li><p><m>p \Longrightarrow (q \vee r)</m> and <m>\neg q \Longrightarrow (\neg p \vee r)</m>.</p></li>
<li><p><m>(p \vee q) \Longrightarrow r</m> and <m>\left( p \Longrightarrow q \right) \land (q \Longrightarrow r)</m>.</p></li>
<li><p><m>\ p \Longrightarrow (q \vee r)</m> and <m>(\neg r) \Longrightarrow (p \Longrightarrow q)</m>.</p></li>
<li><p><m>p \Longrightarrow (q \vee r)</m> and <m>((\neg r) \land p) \Longrightarrow q</m>.</p></li>
</ol>
<ol start="2" type="1">
<li><p>For statements <m>p,q</m>, and <m>r</m>, show that the following compound statements are tautology.</p></li>
</ol>
<ol type="a">
<li><p><m>p \Longrightarrow (p \vee q)</m>.</p></li>
<li><p><m>(p \land \left( p \Longrightarrow q \right)) \Longrightarrow q</m>.</p></li>
<li><p><m>\left( \left( p \Longrightarrow q \right) \land \left( q \Longrightarrow r \right) \right) \Longrightarrow (p \Longrightarrow r)</m>.</p></li>
</ol>
<ol start="3" type="1">
<li><p>For statements <m>p</m> and <m>q</m>, show that <m>\left( p \land \neg q \right) \land (p \land q)</m> is a contradiction.</p></li>
<li><p>Write the contrapositive and the converse of the following conditional statements.</p></li>
</ol>
<ol type="a">
<li><p>If it is cold, then the lake is frozen.</p></li>
<li><p>If Solomon is healthy, then he is happy.</p></li>
<li><p>If it rains, Tigist does not take a walk.</p></li>
</ol>
<ol start="5" type="1">
<li><p>Let <m>p</m> and <m>q</m> be statements. Which of the following implies that <m>p \vee q</m> is false?</p></li>
</ol>
<table>
<tabular>
<row>
<cell><ol type="a">
<li><p><m>\neg p \vee \neg q</m> is false.</p></li>
<li><p><m>\neg p \vee q</m> is true.</p></li>
<li><p><m>\neg p \land \neg q</m> is true.</p></li>
</ol></cell>
<cell><ol start="4" type="a">
<li><p><m>p \Longrightarrow q</m> is true.</p></li>
<li><p><m>p \land q</m> is false.</p></li>
</ol></cell>
</row>
</tabular>
</table>
<ol start="6" type="1">
<li><p>Suppose that the statements <m>p,q,r,</m> and <m>s</m> are assigned the truth values <m>T,F,F,</m> and <m>T</m>, respectively. Find the truth value of each of the following statements.</p></li>
</ol>
<table>
<tabular>
<row>
<cell><ol type="a">
<li><p><m>(p \vee q) \vee r</m>.</p></li>
<li><p><m>p \vee (q \vee r)</m>.</p></li>
<li><p><m>r \Longrightarrow (s \land p)</m>.</p></li>
<li><p><m>p \Longrightarrow (r \Longrightarrow s)</m>.</p></li>
<li><p><m>p \Longrightarrow (r \vee s)</m>.</p></li>
</ol></cell>
<cell><ol start="6" type="a">
<li><p><m>\left( p \vee r \right)\mathbf{\Longleftrightarrow (}r\mathbf{\land}\neg s\mathbf{)}</m><alert>.</alert></p></li>
<li><p><m>\left( s\mathbf{\Longleftrightarrow}p \right) \Longrightarrow (\neg p \vee s)</m>.</p></li>
<li><p><m>\left( q \land \neg s \right) \Longrightarrow (p\mathbf{\Longleftrightarrow}s)</m>.</p></li>
<li><p><m>\left( r \land s \right) \Longrightarrow (p \Longrightarrow (\neg q \vee s))</m>.</p></li>
<li><p><m>\left( p \vee \neg q \right) \vee r \Longrightarrow (s \land \neg s)</m>.</p></li>
</ol></cell>
</row>
</tabular>
</table>
<ol start="7" type="1">
<li><p>Suppose the value of <m>p \Longrightarrow q</m> is <m>T</m>; what can be said about the value of <m>\neg p \land q\mathbf{\Longleftrightarrow}p \vee q</m>?</p></li>
<li><p>a. Suppose the value of <m>p\mathbf{\Longleftrightarrow}q</m> is <m>T</m>; what can be said about the values of <m>p\mathbf{\Longleftrightarrow}\neg q</m> and <m>\neg p\mathbf{\Longleftrightarrow}q</m>?</p></li>
</ol>
<p>b. Suppose the value of <m>p\mathbf{\Longleftrightarrow}q</m> is <m>F</m>; what can be said about the values of <m>p\mathbf{\Longleftrightarrow}\neg q</m> and <m>\neg p\mathbf{\Longleftrightarrow}q</m>?</p>
<ol start="9" type="1">
<li><p>Construct the truth table for each of the following statements.</p></li>
</ol>
<table>
<tabular>
<row>
<cell><ol type="a">
<li><p><m>p \Longrightarrow (p \Longrightarrow q)</m>.</p></li>
<li><p><m>\left( p \vee q \right)\mathbf{\Longleftrightarrow (}q \vee p\mathbf{)}</m><alert>.</alert></p></li>
<li><p><m>p \Longrightarrow \neg(q \land r)</m>.</p></li>
</ol></cell>
<cell><ol start="4" type="a">
<li><p><m>\left( p \Longrightarrow q \right)\mathbf{\Longleftrightarrow (}\neg p \vee q)</m>.</p></li>
<li><p><m>\left( p \Longrightarrow \left( q \land r \right) \right) \vee (\daleth p \land q)</m><m>\left( p \Longrightarrow \left( q \land r \right) \right) \vee (\neg p \land q)</m>.</p></li>
<li><p><m>\left( p \land q \right) \Longrightarrow (\left( q \land \neg q \right) \Longrightarrow (r \land q))</m>.</p></li>
</ol></cell>
</row>
</tabular>
</table>
<ol start="10" type="1">
<li><p>For each of the following determine whether the information given is sufficient to decide the truth value of the statement. If the information is enough, state the truth value. If it is insufficient, show that both truth values are possible.</p></li>
</ol>
<ol type="a">
<li><p><m>(p \Longrightarrow q) \Longrightarrow r</m>, where <m>r = T</m>.</p></li>
<li><p><m>p \land (q \Longrightarrow r)</m>, where <m>q \Longrightarrow r = T</m>.</p></li>
<li><p><m>p \vee (q \Longrightarrow r)</m>, where <m>q \Longrightarrow r = T</m>.</p></li>
<li><p><m>\neg\left( p \vee q \right)\mathbf{\Longleftrightarrow (}\neg p \land \neg q)</m>, where <m>p \vee q = T</m>.</p></li>
<li><p><m>\left( p \Longrightarrow q \right) \Longrightarrow (\neg q \Longrightarrow \neg p)</m>, where <m>q = T</m>.</p></li>
<li><p><m>\left( p \land q \right) \Longrightarrow (p \vee s)</m>, where <m>p = T</m> and <m>s = F</m>.</p></li>
</ol></cell>
</row>

</tabular>
</table>
</subsection>
