<section xmlns:xi="http://www.w3.org/2001/XInclude" xml:id="sec-real-valued-functions-and-their">
<title>Real Valued functions and their properties</title>
<introduction>
<p>After completing this section, the student should be able to:</p>
<ul>
<li><p>perform the four fundamental operations on polynomials</p></li>
<li><p>compose functions to get a new function</p></li>
<li><p>determine the domain of the sum, difference, product and quotient of two functions</p></li>
<li><p>define equality of two functions</p></li>
</ul>
<p>Let <m>f</m> be a function from set <m>A</m> to set <m>B</m>. If <m>B</m> is a subset of the set of real numbers <m>\Re</m>, then <m>f</m> is called a real valued function, and in particular if <m>A</m> is also a subset of <m>\Re</m>, then <m>f:A \rightarrow B</m> is called a real function.</p>
<p><alert>Example 3.10</alert>: 1. The function <m>f:\Re \rightarrow \Re</m> defined by <m>f(x) = x^{2} + 3x + 7</m>, <m>x \in \Re</m> is a real function.</p>
<p>2. The function <m>f:\Re \rightarrow \Re</m> defined as <m>f(x) = \left| x \right|</m> is also a real valued function.</p>
<ul>
<li><p><alert>Operations on functions</alert></p></li>
</ul>
<p>Functions are not numbers. But just as two numbers <m>a</m> and <m>b</m> can be added to produce a new number <m>a + b</m>, so two functions <m>f</m> and <m>g</m> can be added to produce a new function <m>f + g</m>. This is just one of the several operations on functions that we will describe in this section.</p>
<p>Consider functions <m>f</m> and <m>g</m> defined by <m>f(x) = \frac{x - 3}{2}</m> and <m>g(x) = \sqrt{x}</m>. We can make a new function <m>f + g</m> by having it assign to <m>x</m>the value <m>\frac{x - 3}{2} + \sqrt{x}</m>, that is,</p>
<p><m>(f + g)(x) = f(x) + g(x) = \frac{x - 3}{2} + \sqrt{x}</m> .</p>
<table>
<tabular>
<row>
<cell><p><alert>Definition 3.7: Sum, Difference, Product and Quotient of two functions</alert></p>
<p>Let <m>f(x)</m> and <m>g(x)</m> be two functions. We define the following four functions:</p>
<ol type="1">
<li><p><m>(f + g)(x) = f(x) + g(x)</m> The sum of the two functions</p></li>
<li><p><m>(f - g)(x) = f(x) - g(x)</m> The difference of the two functions</p></li>
<li><p><m>(f \cdot g)(x) = f(x)g(x)</m> The product of the two functions</p></li>
<li><p><m>\left( \frac{f}{g} \right)(x) = \frac{f(x)}{g(x)}</m> The quotient of the two functions (provided <m>g(x) \neq 0)</m></p></li>
</ol>
<p>Since an <m>x -</m>value must be an input into both <m>f</m> and <m>g</m>, the domain of <m>(f + g)(x)</m> is the set of all <m>x</m> common to the domain of <m>f</m> and <m>g</m>. This is usually written as <m>\text{Dom}(f + g) = \text{Dom}(f) \cap \text{Dom}(g)</m>. Similar statements hold for the domains of the difference and product of two functions. In the case of the quotient, we must impose the additional restriction that all elements in the domain of <m>g</m> for which <m>g(x) = 0</m> are excluded.</p></cell>
</row>
</tabular>
</table>
<p><alert>Example 3.11</alert>:</p>
<ol type="1">
<li><p>Let <m>f(x) = 3x^{2} + 2</m> and <m>g(x) = 5x - 4</m>. Find each of the following and its domain</p></li>
</ol>
<ol type="a">
<li><p><m>(f + g)(x)</m> b) <m>(f - g)(x)</m> c) <m>(f\text{.}g)(x)</m> d) <m>\left( \frac{f}{g} \right)(x)</m></p></li>
</ol>
<p><alert>Solution</alert>:</p>
<ol type="a">
<li><p><m>(f + g)(x) = f(x) + g(x) = (3x^{2} + 2) + (5x - 4) =</m><m>3x^{2} + 5x - 2</m></p></li>
<li><p><m>(f - g)(x) = f(x) - g(x) = (3x^{2} + 2) - (5x - 4) =</m><m>3x^{2} - 5x + 6</m></p></li>
<li><p><m>(f \cdot g)(x) = (3x^{2} + 2)(5x - 4) =</m><m>\text{15}x^{3} - \text{12}x^{2} + \text{10}x - 8</m></p></li>
<li><p><m>\left( \frac{f}{g} \right)(x) = \frac{f(x)}{g(x)} =</m><m>\frac{3x^{2} + 2}{5x - 4}</m></p></li>
</ol>
<p>We have</p>
<ol start="2" type="1">
<li><p>Let <m>f(x) = \sqrt[4]{x + 1}</m> and <m>g(x) = \sqrt{9 - x^{2}}</m>, with respective domains <m>\lbrack - 1,\infty)</m> and <m>\lbrack - 3,3\rbrack</m>. Find formulas for <m>f + g,\ f - g,\ f \cdot g,\frac{f}{g}</m> and <m>f^{3}</m> and give their domains.</p></li>
</ol>
<p><alert>Solution</alert>:</p>
<table>
<tabular>
<row header="yes">
<cell><alert>Formula Domain</alert></cell>
</row>

<row>
<cell><p><m>(f + g)(x) = f(x) + g(x) = \sqrt[4]{x + 1} + \sqrt{9 - x^{2}}</m> <m>\lbrack - 1,\ 3\rbrack</m></p>
<p><m>(f - g)(x) = f(x) - g(x) = \sqrt[4]{x + 1} - \sqrt{9 - x^{2}}</m> <m>\lbrack - 1,\ 3\rbrack</m></p>
<p><m>(f \cdot g)(x) = f(x) \cdot g(x) = \sqrt[4]{x + 1} \cdot \sqrt{9 - x^{2}}</m> <m>\lbrack - 1,\ 3\rbrack</m></p>
<p><m>\left( \frac{f}{g} \right)(x) = \frac{f(x)}{g(x)} = \frac{\sqrt[4]{x + 1}}{\sqrt{9 - x^{2}}}</m> <m>\lbrack - 1,\ 3)</m></p>
<p><m>f^{3}(x) = \left( f(x) \right)^{3} = \left( \sqrt[4]{x + 1} \right)^{3} = \left( x + 1 \right)^{\frac{3}{4}}</m> <m>\lbrack - 1,\infty)</m></p></cell>
</row>
</tabular>
</table>
<p>There is yet another way of producing a new function from two given functions.</p>
<table>
<tabular>
<row>
<cell><p><alert>Definition 3.8: (Composition of functions)</alert></p>
<p>Given two functions <m>f(x)</m> and <m>g(x)</m>, the composition of the two functions is denoted by <m>f \circ g</m> and is defined by:</p>
<p><m>(f \circ g)(x) = f\lbrack g(x)\rbrack</m>.</p>
<p><m>(f \circ g)(x)</m> is read as <m>\text{f\}\ \{}</m> composed with <m>g</m> of <m>x\text{\}\ \{}</m>.<m></m>The domain of <m>f \circ g</m> consists of those <m>x^{&#39;}</m>s in the domain of <m>g</m> whose range values are in the domain of <m>f</m>, i.e. those <m>x^{&#39;}</m>s for which <m>g(x)</m> is in the domain of <m>f</m>.</p></cell>
</row>
</tabular>
</table>
<p><alert>Example 3.12</alert>:</p>
<ol type="1">
<li><p>Suppose <m>f = \left\{ (2,z),(3,q) \right\}</m> and <m>g = \left\{ (a,2),(b,3),(c,5) \right\}</m>. The function <m>(f \circ g)(x) = f(g(x))</m> is found by taking elements in the domain of <m>g</m> and evaluating as follows:</p></li>
</ol>
<p>If we attempt to find <m>f(g(c))</m> we get <m>f(5)</m>, but 5 is not in the domain of <m>f(x)</m> and so we cannot find <m>(f \circ g)(c)</m>. Hence, <m>f \circ g = \left\{ (a,z),(b,q) \right\}</m>. The figure below illustrates this situation.</p>
<ol start="2" type="1">
<li><p>Given <m>f(x) = 5x^{2} - 3x + 2</m> and <m>g(x) = 4x + 3</m>, find</p></li>
</ol>
<ol type="a">
<li><p><m>(f \circ g)( - 2)</m> b) <m>(g \circ f)(2)</m> c) <m>(f \circ g)(x)</m> d) <m>(g \circ f)(x)</m></p></li>
</ol>
<p><alert>Solution</alert>:</p>
<ol type="a">
<li><p><m>(f \circ g)( - 2) = f(g( - 2))</m>…… First evaluate <m>g( - 2) = 4( - 2) + 3 = - 5</m></p></li>
</ol>

<p><m>= f( - 5)</m></p>
<p><m>= 5( - 5)^{2} - 3( - 5) + 2 = \text{142}</m></p>

<ol start="2" type="a">
<li><p><m>(g \circ f)(2) = g(f(2))</m>…….First evaluate <m>f(2) = 5(2)^{2} - 3(2) + 2 = \text{16}</m></p></li>
</ol>
<p><m>= g(\text{16})</m></p>
<p><m>= 4(\text{16}) + 3 = \text{67}</m></p>
<ol start="3" type="a">
<li><p><m>(f \circ g)(x) = f(g(x))</m>……. But <m>g(x) = 4x + 3</m></p></li>
</ol>

<p><m>= f(4x + 3)</m></p>
<p><m>= 5(4x + 3)^{2} - 3(4x + 3) + 2</m></p>
<p><m>= \text{80}x^{2} + \text{108}x + \text{38}</m></p>

<ol start="4" type="a">
<li><p><m>(g \circ f)(x) = g(f(x))</m>……. But <m>f(x) = 5x^{2} - 3x + 2</m></p></li>
</ol>

<p><m>= g(5x^{2} - 3x + 2)</m></p>
<p><m>= 4(5x^{2} - 3x + 2) + 3</m></p>
<p><m>= \text{20}x^{2} - \text{12}x + \text{11}</m></p>

<ol start="3" type="1">
<li><p>Given <m>f(x) = \frac{x}{x + 1}</m> and <m>g(x) = \frac{2}{x - 1}</m>, find</p></li>
</ol>
<ol type="a">
<li><p><m>(f \circ g)(x)</m> and its domain b) <m>(g \circ f)(x)</m> and its domain</p></li>
</ol>
<p><alert>Solution</alert>: a) <m>(f \circ g)(x) = f\left( \frac{2}{x - 1} \right) = \frac{\frac{2}{x - 1}}{\frac{2}{x - 1} + 1} = \frac{2}{x + 1}</m>. Thus, <m>\text{Dom}(f \circ g) = \left\{ x:x \neq \pm 1 \right\}</m>.</p>
<ol start="2" type="a">
<li><p><m>(g \circ f)(x) = g(f(x)) = \frac{2}{\frac{x}{x + 1} - 1} = - 2x - 2</m>. Since <m>x</m> must first be an input into <m>f(x)</m> and so must be in the domain of <m>f</m>, we see that <m>\text{Dom}(g \circ f) = \left\{ x:x \neq - 1 \right\}</m>.</p></li>
</ol>
<ol start="4" type="1">
<li><p>Let <m>f(x) = \frac{6x}{x^{2} - 9}</m> and <m>g(x) = \sqrt{3x}</m>. Find <m>(f \circ g)(\text{12})</m> and <m>(g \circ f)(x)</m> and its domain.</p></li>
</ol>
<p><alert>Solution</alert>: We have <m>(f \circ g)(\text{12}) = f(g(\text{12})) = f(\sqrt{\text{36}}) = f(6) = \frac{\text{36}}{\text{27}} = \frac{4}{3}</m>.</p>

<p><m>(f \circ g)(x) = f(g(x)) = f(\sqrt{3x}) = \frac{6\sqrt{3x}}{(\sqrt{3x})^{2} - 9} = \frac{6\sqrt{3x}}{3x - 9} = \frac{2\sqrt{3x}}{x - 3}</m>.</p>

<p>The domain of <m>f \circ g</m> is <m>\lbrack 0,3) \cup (3,\infty)</m>.</p>
<p>We now explore the meaning of equality of two functions. Let <m>f:A \rightarrow B</m> and <m>g:A \rightarrow B</m> be two functions. Then, <m>f</m> and <m>g</m> are subsets of <m>A \times B</m>. Suppose <m>f = g</m>. Let <m>x</m> be any element of <m>A</m>. Then, <m>(x,f(x)) \in f = g</m> and thus <m>(x,f(x)) \in g</m>. Since <m>g</m> is a function and <m>(x,f(x)),</m><m>(x,g(x)) \in g</m>, we must have <m>f(x) = g(x)\text{.}</m> Conversely, assume that <m>g(x) = f(x)</m> for all <m>x \in A</m>. Let <m>(x,y) \in f</m>. Then, <m>y = f(x) = g(x)</m>. Thus, <m>(x,y) \in g</m>, which implies that <m>f \subseteq g</m>. Similarly, we can show that <m>g \subseteq f</m>. It now follows that <m>f = g</m>. Thus two functions <m>f:A \rightarrow B</m> and <m>g:A \rightarrow B</m> are equal if and only if <m>f(x) = g(x)</m> for all <m>x \in A</m>. In general we have the following definition.</p>
<table>
<tabular>
<row>
<cell><p><alert>Definition 3.9: (Equality of functions)</alert></p>
<p>Two functions are said to be equal if and only if the following two conditions hold:</p>
<ol type="i">
<li><p>The functions have the same domain;</p></li>
<li><p>Their functional values are equal at each element of the domain.</p></li>
</ol></cell>
</row>
</tabular>
</table>
<p><alert>Example 3.13</alert>:</p>
<ol type="1">
<li><p>Let <m>f:Z \rightarrow Z^{+} \cup \left\{ 0 \right\}</m> and <m>g:Z \rightarrow Z^{+} \cup \left\{ 0 \right\}</m> be defined by <m>f = \left\{ (n,n^{2}):n \in Z \right\}</m> and <m>g = \left\{ (n,\left| n \right|^{2}):n \in Z \right\}</m>. Now, for all <m>n \in Z</m>, <m>f(n) = n^{2} = \left| n \right|^{2} = g(n)</m>. Thus, <m>f = g</m>.</p></li>
<li><p>Let <m>f(x) = \frac{x^{2} - \text{25}}{x - 5},\ x \in \Re\{ 5</m>, and <m>g(x) = x + 5,\ x \in \Re</m>. The function <m>f</m> and <m>g</m> are not equal because <m>\text{Dom}(f) \neq \text{Dom}(g)\text{.}</m></p></li>
</ol>
<p><alert>Exercise 3.2</alert></p>
<ol type="1">
<li><p>For <m>f(x) = x^{2} + x</m> and <m>g(x) = \frac{2}{x + 3}</m>, find each value:</p></li>
</ol>
<ol type="a">
<li><p><m>(f - g)(2)</m> c) <m>g^{2}(3)</m> e) <m>(g \circ f)(1)</m></p></li>
<li><p><m>\left( \frac{f}{g} \right)(1)</m> d) <m>(f \circ g)(1)</m> f) <m>(g \circ g)(3)</m></p></li>
</ol>
<ol start="2" type="1">
<li><p>If <m>f(x) = x^{3} + 2</m> and <m>g(x) = \frac{2}{x - 1}</m>, find a formula for each of the following and state its domain.</p></li>
</ol>
<ol type="a">
<li><p><m>(f + g)(x)</m> c) <m>\left( \frac{g}{f} \right)(x)</m></p></li>
<li><p><m>(f \circ g)(x)</m> d) <m>(g \circ f)(x)</m></p></li>
</ol>
<ol start="3" type="1">
<li><p>Let <m>f(x) = x^{2}</m> and <m>g(x) = \sqrt{x}</m>.</p></li>
</ol>
<ol type="a">
<li><p>Find <m>(f \circ g)(x)</m> and its domain.</p></li>
<li><p>Find <m>(g \circ f)(x)</m> and its domain</p></li>
<li><p>Are <m>(f \circ g)(x)</m> and <m>(g \circ f)(x)</m> the same functions? Explain.</p></li>
</ol>
<ol start="4" type="1">
<li><p>Let <m>f(x) = 5x - 3</m>. Find <m>g(x)</m> so that <m>(f \circ g)(x) = 2x + 7</m>.</p></li>
<li><p>Let <m>f(x) = 2x + 1\text{.}</m> Find <m>g(x)</m> so that <m>(f \circ g)(x) = 3x - 1</m>.</p></li>
<li><p>If <m>f</m> is a real function defined by <m>f(x) = \frac{x - 1}{x + 1}</m>. Show that <m>f(2x) = \frac{3f(x) + 1}{f(x) + 3}</m>.</p></li>
<li><p>Find two functions <m>f</m> and <m>g</m> so that the given function <m>h(x) = (f \circ g)(x)</m>, where</p></li>
</ol>
<ol type="a">
<li><p><m>h(x) = (x + 3)^{3}</m> c) <m>h(x) = \frac{1}{x} + 6</m></p></li>
<li><p><m>h(x) = \sqrt{5x - 3}</m> d) <m>h(x) = \frac{1}{x + 6}</m></p></li>
</ol>
<ol start="8" type="1">
<li><p>Let <m>f(x) = 4x - 3,\ g(x) = \frac{1}{x}</m> and <m>h(x) = x^{2} - x</m>. Find</p></li>
</ol>
<ol type="a">
<li><p><m>f(5x + 7)</m> c) <m>f(g(h(3)))</m> e) <m>f(x + a)</m></p></li>
<li><p><m>5f(x) + 7</m> d) <m>f(1) \cdot g(2) \cdot h(3)</m> f) <m>f(x) + a</m></p></li>
</ol>

</introduction>

</section>