<section xmlns:xi="http://www.w3.org/2001/XInclude" xml:id="sec-types-of-functions-and-inverse">
<title>Types of functions and inverse of a function</title>
<introduction>
<p>After completing this section, the student should be able to:</p>
<ul>
<li><p>define one to oneness and ontoness of a function</p></li>
<li><p>check invertibility of a function</p></li>
<li><p>find the inverse of an invertible function</p></li>
</ul>
<p>In this section we shall study some important types of functions.</p>
<ul>
<li><p><alert>One to One functions</alert></p></li>
</ul>
<table>
<tabular>
<row>
<cell><alert>Definition 3.10:</alert> A function <m>f:A \rightarrow B</m> is called <alert>one to one</alert>, often written 1 – 1, if and only if for all <m>x_{1},x_{2} \in A</m>, <m>f(x_{1}) = f(x_{2})</m> implies <m>x_{1} = x_{2}</m>. In words, no two elements of <m>A</m> are mapped to one element of <m>B</m>.</cell>
</row>
</tabular>
</table>
<p><alert>Example 3.14</alert>:</p>
<ol type="1">
<li><p>If we consider the sets <m>A = \left\{ 1,2,3,\cdots,6 \right\}</m> and <m>B = \left\{ 7,a,b,c,d,8,e \right\}</m> and if <m>f =</m><m>(2,a),</m><m>(3,b)</m>, <m>(4,b),(5,c),(6,8)</m> and <m>g = \left\{ (1,7),(2,a),(3,b),(4,c),(5,8),(6,d) \right\}</m>, then both <m>f</m> and <m>g</m> are functions from <m>A</m> into <m>B</m>. Observe that <m>f</m> is not a 1 – 1 function because <m>f(3) = f(4)</m> but <m>3 \neq 4</m>. However, <m>g</m> is a 1 – 1 function.</p></li>
<li><p>Let <m>A = \left\{ 1,2,3,4 \right\}</m> and <m>B = \left\{ 1,4,7,8 \right\}</m>. Consider the functions</p></li>
</ol>
<ol type="i">
<li><p><m>f:A \rightarrow B</m> defined as <m>f(1) = 1,\ f(2) = 4,\ f(3) = 4,\ f(4) = 8</m></p></li>
<li><p><m>g:A \rightarrow B</m> defined as <m>f(1) = 4,\ f(2) = 7,\ f(3) = 1,\ f(4) = 8</m></p></li>
</ol>

<p>Then, <m>f</m> is not 1 – 1, but <m>g</m> is a 1 – 1 function.</p>

<ul>
<li><p><alert>Onto functions</alert></p></li>
</ul>
<table>
<tabular>
<row>
<cell><alert>Definition 3.11:</alert> Let <m>f</m> be a function from a set <m>A</m> into a set <m>B</m>. Then <m>f</m> is called an <alert>onto function(or</alert> <m>f</m><alert>maps onto</alert> <m>B)</m> if every element of <m>B</m> is an image of some element in <m>A</m>, i.e, <m>\text{Range}(f) = B\text{.}</m></cell>
</row>
</tabular>
</table>
<p><alert>Example 3.15</alert>:</p>
<ol type="1">
<li><p>Let <m>A = \left\{ 1,2,3 \right\}</m>and <m>B = \left\{ 1,4,5 \right\}</m>. The function <m>f:A \rightarrow B</m> defined by <m>f(1) = 1</m>, <m>f(2) = 5</m>, <m>f(3) = 1</m> is not onto because there is no element in <m>A</m>, whose image under <m>f</m> is 4. The function <m>g:A \rightarrow B</m> given by <m>g = \left\{ (1,4),(2,5),(3,1) \right\}</m> is onto because each element of <m>B</m> is an image of at least one element of <m>A</m> .</p></li>
</ol>
<p>Note that if <m>A</m> is a non-empty set, the function <m>i_{A}:A \rightarrow A</m> defined by <m>i_{A}(x) = x</m> for all <m>x \in A</m> is a 1 – 1 function from <m>A</m> onto <m>A</m>. <m>i_{A}</m> is called the <alert>identity map</alert> on <m>A</m>.</p>
<ol start="2" type="1">
<li><p>Consider the relation <m>f</m> from <m>Z</m> into <m>Z</m> defined by <m>f(n) = n^{2}</m> for all <m>n \in Z</m>. Now, domain of <m>f</m> is <m>Z</m>. Also, if <m>n = n^{&#39;}</m>, then <m>n^{2} = (n^{&#39;})^{2}</m>, i.e. <m>f(n) = f(n^{&#39;})</m>. Hence, <m>f</m> is well defined and is a function. However, <m>f(1) = 1 = f( - 1)</m> and <m>1 \neq - 1</m>, which implies that <m>f</m> is not 1 – 1. For all <m>n \in Z</m>, <m>f(n)</m> is a non-negative integer. This shows that a negative integer has no preimage. Hence, <m>f</m> is not onto. Note that <m>f</m> is onto <m>\left\{ 0,1,4,9,\cdots \right\}</m>.</p></li>
<li><p>Consider the relation <m>f</m> from <m>Z</m> into <m>Z</m> defined by <m>f(n) = 2n</m> for all <m>n \in Z</m>. As in the previous example, we can show that <m>f</m> is a function. Let <m>n,n^{&#39;} \in Z</m> and suppose that <m>f(n) = f(n^{&#39;})</m>. Then <m>2n = 2n^{&#39;}</m> and thus <m>n = n^{&#39;}</m>. Hence, <m>f</m> is 1 – 1. Since for all <m>n \in Z</m>, <m>f(n)</m> is an even integer; we see that an odd integer has no preimage. Therefore, <m>f</m> is not onto.</p></li>
</ol>
<ul>
<li><p><alert>1 – 1 Correspondence</alert></p></li>
</ul>
<table>
<tabular>
<row>
<cell><alert>Definition 3.12:</alert> A function <m>f:A \rightarrow B</m> is said to be a 1 – 1 correspondence if <m>f</m> is both 1 – 1 and onto.</cell>
</row>
</tabular>
</table>
<p><alert>Example 3.16</alert>:</p>
<ol type="1">
<li><p>Let <m>A = \left\{ 0,\ 1,\ 2,\ 3,\ 4,\ 5 \right\}</m> and <m>B = \left\{ 0,\ 5,\ \text{10},\ \text{15},\ \text{20},\ \text{25} \right\}</m>. Suppose <m>f:A \rightarrow B</m> given by <m>f(x) = 5x</m> for all <m>x \in A</m>. One can easily see that every element of <m>B</m> has a preimage in <m>A</m> and hence <m>f</m> is onto. Moreover, if <m>f(x) = f(y)</m>, then <m>5x = 5y</m>, i.e. <m>x = y</m>. Hence, <m>f</m> is 1 – 1. Therefore, <m>f</m> is a 1 – 1 correspondence between <m>A</m> and <m>B</m>.</p></li>
<li><p>Let <m>A</m> be a finite set. If <m>f:A \rightarrow A</m> is onto, then it is one to one.</p></li>
</ol>
<p><alert>Solution</alert>: Let <m>A = \left\{ a_{1},a_{2},\cdots,a_{n} \right\}</m>. Then <m>\text{Range}(f) = \left\{ f(a_{1}),f(a_{2}),\cdots,f(a_{n}) \right\}</m>. Since <m>f</m> is onto we have <m>\text{Range}(f) = A</m>.Thus, <m>A = \left\{ f(a_{1}),f(a_{2}),\cdots,f(a_{n}) \right\}</m>, which implies that <m>f(a_{1})</m>, <m>f(a_{2})</m>, <m>\cdots</m>, <m>f(a_{n})</m> are all distinct. Hence, <m>a_{i} \neq a_{j}</m> implies <m>f(a_{i}) \neq f(a_{j})</m> for all <m>1 \leq i,j \leq n</m>. Therefore, <m>f</m> is 1 – 1.</p>
<ul>
<li><p><alert>Inverse of a function</alert></p></li>
</ul>
<p>Since a function is a relation , the inverse of a function <m>f</m> is denoted by <m>f^{- 1}</m> and is defined by:</p>

<p><m>f^{- 1} = \left\{ (y,x):(x,y) \in f \right\}</m></p>

<p>For instance, if <m>f = \left\{ (2,4),(3,6),(1,7) \right\}</m>, then <m>f^{- 1} = \left\{ (4,2),(6,3),(7,1) \right\}</m>. Note that the inverse of a function is not always a function. To see this consider the function <m>f =</m><m>(5,4)</m>. Then, <m>f^{- 1} = \left\{ (4,2),(6,3),(4,5) \right\}</m>, which is not a function.</p>
<p>As we have seen above not all functions have an inverse, so it is important to determine whether or not a function has an inverse before we try to find the inverse. If the function does not have an inverse, then we need to realize that it does not have an inverse so that we do not waste our time trying to find something that does not exist.</p>
<p>A one to one function is special because only one to one functions have inverse. If a function is one to one, to find the inverse we will follow the steps below:</p>
<ol type="1">
<li><p>Interchange <m>x</m> and <m>y</m> in the equation <m>y = f(x)</m></p></li>
<li><p>Solving the resulting equation for <m>y</m>, we will obtaining the inverse function.</p></li>
</ol>
<p>Note that the domain of the inverse function is the range of the original function and the range of the inverse function is the domain of the original function.</p>
<p><alert>Example 3.17</alert>:</p>
<ol type="1">
<li><p>Given <m>y = f(x) = x^{3}</m>. Find <m>f^{- 1}</m> and its domain.</p></li>
</ol>
<p><alert>Solution</alert>: We begin by interchanging <m>x</m> and <m>y</m>, and we solve for <m>y</m>.</p>
<table>
<tabular>
<row header="yes">
<cell></cell>
<cell>Interchange <m>x</m> and <m>y</m></cell>
</row>

<row>
<cell></cell>
<cell>Take the cube root of both sides</cell>
</row>
<row>
<cell></cell>
<cell>This is the inverse of the function</cell>
</row>
</tabular>
</table>

<p>Thus, <m>f^{- 1}(x) = \sqrt[3]{x}</m>. The domain of <m>f^{- 1}</m> is the set of all real numbers.</p>

<ol start="2" type="1">
<li>
<p>Let <m>y = f(x) = \frac{x}{x + 2}</m>. Find <m>f^{- 1}(x)</m>.</p>
</li>
</ol>
<p><alert>Solution</alert>: Again we begin by interchanging <m>x</m> and <m>y</m>, and then we solve for <m>y</m>.</p>

<p><m>y = \frac{x}{x + 2}</m> Interchange <m>x</m> and <m>y</m></p>
<p><m>x = \frac{y}{y + 2}</m> Solving for <m>y</m></p>
<p><m>x(y + 2) = y\  \Leftrightarrow \ \text{xy} + 2x = y\  \Leftrightarrow \ 2x = y(1 - x)\  \Leftrightarrow y = \frac{2x}{1 - x}</m></p>

<p>Thus, <m>f^{- 1}(x) = \frac{2x}{1 - x}</m>.</p>
<p><alert>Remark</alert>: Even though, in general, we use an exponent of <m>- 1</m> to indicate a reciprocal, inverse function notation is an exception to this rule. Please be aware that <m>f^{- 1}(x)</m> is not the reciprocal of <m>f</m>. That is,</p>

<p><m>f^{- 1}(x) \neq \frac{1}{f(x)}</m></p>

<p>If we want to write the reciprocal of the function <m>f(x)</m> by using a negative exponent, we must write</p>

<p><m>\frac{1}{f(x)} = \left\lbrack f(x) \right\rbrack^{- 1}</m>.</p>

<p><alert>Exercise 3.3</alert></p>
<ol type="1">
<li><p>Consider the function <m>f = \left\{ (x,x^{2}):x \in S \right\}</m> from <m>S = \left\{ - 3, - 2, - 1,0,1,2,3 \right\}</m> into <m>Z</m>. Is <m>f</m> one to one? Is it onto?</p></li>
<li><p>Let <m>A = \left\{ 1,2,3 \right\}</m>. List all one to one functions from <m>A</m> onto <m>A</m>.</p></li>
<li><p>Let <m>f:A \rightarrow B</m>. Let <m>f^{}</m> be the inverse relation, i.e. <m>f^{} = \left\{ (y,x) \in B \times A:f(x) = y \right\}</m>.</p></li>
</ol>
<ol type="a">
<li><p>Show by an example that <m>f^{}</m> need not be a function.</p></li>
<li><p>Show that <m>f^{}</m> is a function from <m>\text{Range}(f)</m> into <m>A</m> if and only if <m>f</m> is 1 – 1.</p></li>
<li><p>Show that <m>f^{}</m> is a function from <m>B</m> into <m>A</m> if and only if <m>f</m> is 1 – 1 and onto.</p></li>
<li><p>Show that if <m>f^{}</m> is a function from <m>B</m> into <m>A</m>, then <m>f^{- 1} = f^{}</m>.</p></li>
</ol>
<ol start="4" type="1">
<li><p>Let <m>A = \left\{ x \in \Re:0 \leq x \leq 1 \right\}</m> and <m>B = \left\{ x \in \Re:5 \leq x \leq 8 \right\}</m>. Show that <m>f:A \rightarrow B</m> defined by <m>f(x) = 5 + (8 - 5)x</m> is a 1 – 1 function from <m>A</m> onto <m>B</m>.</p></li>
<li><p>Which of the following functions are one to one?</p></li>
</ol>
<ol type="a">
<li><p><m>f:\Re \rightarrow \Re</m> defined by <m>f(x) = 4,\ x \in \Re</m></p></li>
<li><p><m>f:\Re \rightarrow \Re</m> defined by <m>f(x) = 6x - 1,\ x \in \Re</m></p></li>
<li><p><m>f:\Re \rightarrow \Re</m> defined by <m>f(x) = x^{2} + 7,\ x \in \Re</m></p></li>
<li><p><m>f:\Re \rightarrow \Re</m> defined by <m>f(x) = x^{3},\ x \in \Re</m></p></li>
<li><p><m>f:\Re\{ 7 \rightarrow \Re</m> defined by <m>f(x) = \frac{2x + 1}{x - 7},\ x \in \Re\{ 7</m></p></li>
</ol>
<ol start="6" type="1">
<li><p>Which of the following functions are onto?</p></li>
</ol>
<ol type="a">
<li><p><m>f:\Re \rightarrow \Re</m> defined by <m>f(x) = \text{115}x + \text{49},\ x \in \Re</m></p></li>
<li><p><m>f:\Re \rightarrow \Re</m> defined by <m>f(x) = \left| x \right|,\ x \in \Re</m></p></li>
<li><p><m>f:\Re \rightarrow \Re</m> defined by <m>f(x) = \sqrt{x^{2}},\ x \in \Re</m></p></li>
<li><p><m>f:\Re \rightarrow \Re</m> defined by <m>f(x) = x^{2} + 4,\ x \in \Re</m></p></li>
</ol>
<ol start="7" type="1">
<li><p>Find <m>f^{- 1}(x)</m> if</p></li>
</ol>
<ol type="a">
<li><p><m>f(x) = 7x - 6</m> d) <m>f(x) = \frac{4 - x}{3x}</m> g) <m>f(x)\text{==} - (x + 2)^{2} - 1</m></p></li>
<li><p><m>f(x) = \frac{2x - 9}{4}</m> e) <m>f(x) = \frac{5x + 3}{1 - 2x}</m> h) <m>f(x) = \frac{2x}{1 + x}</m></p></li>
<li><p><m>f(x) = 1 - \frac{3}{x}</m> f) <m>f(x) = \sqrt[3]{x + 1}</m></p></li>
</ol>

</introduction>

</section>