<stack-static>
<statement><div><p>Find the four fourth roots of <m>z={0} + {-4}i</m>. Give all roots using principal argument!.</p><p>Recall that <m>\sqrt[n]{r}</m> is entered as <m>r^{1/n}</m>.</p>
<p><em>Note: Write <m>z</m> in exponential form first using principal argument, and the four fourth roots of <m>z</m> in trigonometric form</em></p>
<br/><m>r =</m>  <fillin characters="8" name="ans1"/> and <m>\theta</m> = <fillin characters="8" name="ans2"/> <nbsp/>
<br/><m>z =</m> <fillin characters="15" name="ans3"/>
<p/>
<br/>The four fourth roots of <m>z</m> in trigonometric form are:
<br/><m>z_{0}</m> = <fillin characters="18" name="ans4"/> 
<br/><m>z_{1}</m> = <fillin characters="18" name="ans5"/> 
<br/><m>z_{2}</m> = <fillin characters="18" name="ans6"/> 
<br/><m>z_{3}</m> = <fillin characters="18" name="ans7"/> 
<p> </p></div></statement>
<solution><div><h3>Worked solution</h3>
<p>Find the three square roots of  <m>z={0} {-} {4}i</m>. Give all roots using principal argument!. </p>
<p><em>Note:  Write <m>z</m> in exponential form first using its principal argument, and the three square roots of <m>z</m> in trigonometric form. <br/>Recall that <m>\sqrt[n]{r}</m> is entered as <m>r^{1/n}</m>.</em></p>
<p>Recall that if <m>z=x+iy</m>, <m>r = |z| = \sqrt{x^{2}+y^{2}}</m> and depending on the quadrant in which your complex number lies, <m>\theta</m> is obtained from <m>\tan^{-1}(y/x)</m>.</p>
<p><span/></p>
<p>In this case, your complex number lies in Quadrant 3 where  <m>\tan^{-1}(y/x) = {\frac{\pi}{2}}</m>  and <m>\theta = \pi+{\frac{\pi}{2}} = {-\frac{\pi}{2}}</m>. </p>
<p><span/></p>
<p>So <m>r = {4}</m> and <m>\theta = {-\frac{\pi}{2}}</m> and hence in  exponential form, <m>z=\displaystyle {4} e^{i({-\frac{\pi}{2}})}</m>.</p>
<p> </p>
<p>We apply the following formula to get the roots, <m> z_{k}= \displaystyle |z|^{\frac{1}{n}}e^{({\frac{\Theta}{n}}+{\frac{2 \pi k}{n}})i}</m> where <m>n=4</m>, and <m>k=0,1,2,3</m>. So,</p>
 
<p><md>
<mrow>z_{k}= \displaystyle {4}^{\frac{1}{4}}e^{({-\frac{\pi}{8}}+{\frac{\pi k}{2}})i}</mrow>
</md></p>
 
<p><md>
<mrow>\text{For} \; \amp  k=0, \amp  \displaystyle z_{0}= \displaystyle {\sqrt{2}} e^{{-\frac{\pi}{8}}i}={\sqrt{2}} \left( \cos({-\frac{\pi}{8}}) + i \sin({-\frac{\pi}{8}}) \right)</mrow>
<mrow>\text{For} \; \amp  k=1, \amp  \displaystyle z_{1}= \displaystyle {\sqrt{2}} e^{{\frac{3 \pi}{8}}i} = {\sqrt{2}} \left( \cos({\frac{3 \pi}{8}}) + i \sin({\frac{3 \pi}{8}}) \right)</mrow>
<mrow>\text{For} \; \amp  k=2, \amp  \displaystyle z_{2}= \displaystyle {\sqrt{2}} e^{{\frac{7 \pi}{8}}i} = {\sqrt{2}} \left( \cos({\frac{7 \pi}{8}}) + i \sin({\frac{7 \pi}{8}}) \right)</mrow>
<mrow>\text{For} \; \amp  k=3, \amp  \displaystyle z_{3}= \displaystyle {\sqrt{2}} e^{{-\frac{5 \pi}{8}}i} = {\sqrt{2}} \left( \cos({-\frac{5 \pi}{8}}) + i \sin({-\frac{5 \pi}{8}}) \right)</mrow>
</md></p></div></solution>
<answer><p><m>4</m></p></answer>
<answer><p><m>-\frac{\pi}{2}</m></p></answer>
<answer><p><m>4 e^{\left(-\frac{\pi}{2}\right) \mathrm{i}}</m></p></answer>
<answer><p><m>4^{\frac{1}{4}} \left(\cos \left( -\frac{\pi}{8} \right)+\mathrm{i} \sin \left( -\frac{\pi}{8} \right)\right)</m></p></answer>
<answer><p><m>4^{\frac{1}{4}} \left(\cos \left( \frac{3 \pi}{8} \right)+\mathrm{i} \sin \left( \frac{3 \pi}{8} \right)\right)</m></p></answer>
<answer><p><m>4^{\frac{1}{4}} \left(\cos \left( \frac{7 \pi}{8} \right)+\mathrm{i} \sin \left( \frac{7 \pi}{8} \right)\right)</m></p></answer>
<answer><p><m>4^{\frac{1}{4}} \left(\cos \left( -\frac{5 \pi}{8} \right)+\mathrm{i} \sin \left( -\frac{5 \pi}{8} \right)\right)</m></p></answer>
</stack-static>