<stack-static>
<statement><span><br/> Find the foci, and eccentricity of the ellipse <m> {3\cdot y^2-18\cdot y+x^2+8\cdot x+42=0} </m>.
<br/> Hint: Type <c>sqrt(x)</c> for <m>\sqrt{x}</m>.
<br/> a) Focus 
<br/><m> F_{1}=</m>  <fillin characters="7" name="ans1"/>    <m> F_{2}=</m>  <fillin characters="7" name="ans2"/>    
<br/> b) Eccentricity
<br/> <m> e=</m>  <fillin characters="15" name="ans3"/>    </span></statement>
<solution><span><br/><alert>Worked solution</alert>
<br/> Find the foucs, and eccentricity of the ellipse <m> {3\cdot y^2-18\cdot y+x^2+8\cdot x+42=0} </m>.
<br/> The equation of a ellipse in standard form follows:
 <br/><me> \frac{(x-h)^2}{a^2} + \frac{(y-k)^2}{b^2} = 1</me>
<br/> Here the center is <m>(h, k)</m> and the eccentricity is <m> e =\frac{c}{a}</m>
<br/> If <m> a &gt; b </m>, Foci: <m> F_{1} (h-c, k) </m> and  <m> F_{2}  (h+c, k) </m>
<br/> <m> (H): {3\cdot y^2-18\cdot y+x^2+8\cdot x+42=0} </m>
<br/> <m> \Leftrightarrow {\frac{1}{3}} \cdot ({x^2+8\cdot x+16}) + {1} \cdot ({y^2-6\cdot y+9}) -{\frac{1}{3}}  =0 </m>
<br/> <m> \Leftrightarrow  {{\left(y-3\right)}^2+\frac{{\left(x+4\right)}^2}{3}=\frac{1}{3}} </m>
<br/> <m> \Leftrightarrow   \frac{(x-({-4}))^2}{1} + \frac{(y-({3}))^2}{\frac{1}{3}} = 1</m>
<br/>  For <m> a= {1} </m> and <m> b = {\frac{1}{\sqrt{3}}}</m>, <m> h={-4} </m> and <m> k={3} </m>
<br/> <m> c^2 = a^2-b^2= {\frac{2}{3}} \implies c = {\frac{\sqrt{2}}{\sqrt{3}}}</m>
<br/> Since <m> a &gt; b </m> It follows that
<br/> a) Focus : <m> F_{1}({-\frac{\sqrt{2}}{\sqrt{3}}-4}, {3})</m> and <m> F_{2} ({\frac{\sqrt{2}}{\sqrt{3}}-4}, {3}) </m>

<br/> b) Eccentricity <m> e={\frac{\sqrt{2}}{\sqrt{3}}}</m></span></solution>
<answer><p><m>\left(\begin{array}{c} -\frac{\sqrt{2}}{\sqrt{3}}-4 \\ 3 \end{array}\right)</m></p></answer>
<answer><p><m>\left(\begin{array}{c} \frac{\sqrt{2}}{\sqrt{3}}-4 \\ 3 \end{array}\right)</m></p></answer>
<answer><p><m>\frac{\sqrt{2}}{\sqrt{3}}</m></p></answer>
</stack-static>