<stack-static>
<statement><div><p>Find the two square  roots of <m>z={-\frac{9}{\sqrt{2}}+\frac{9}{\sqrt{2}}}i</m>. Give all roots using principal argument!</p>
<p><em>Note:  Write <m>z</m> in exponential form first using its principal argument, and the two square roots of <m>z</m> in trigonometric form. <br/>Recall that <m>\sqrt[n]{r}</m> is entered as <m>r^{1/n}</m>.</em></p>
<p>r = <fillin characters="8" name="ans1"/><nbsp/> and <m>\theta</m> = <fillin characters="8" name="ans2"/> <nbsp/></p>
<p>z = <fillin characters="15" name="ans3"/></p>
<p/>
<p> The two square roots of <m>z</m> in trigonometric are;</p>
<p><m>z_{0}</m> = <fillin characters="18" name="ans4"/> </p>
<p><m>z_{1}</m> = <fillin characters="18" name="ans5"/> </p>
<p/></div></statement>
<solution><div><h3>Worked solution</h3>
<p>Find the two square roots of  <m>z={-\frac{9}{\sqrt{2}}} {+} {\frac{9}{\sqrt{2}}}i</m>. Give all roots using principal argument!. </p>
<p><em>Note:  Write <m>z</m> in exponential form first using its principal argument, and the three square roots of <m>z</m> in trigonometric form. <br/>Recall that <m>\sqrt[n]{r}</m> is entered as <m>r^{1/n}</m>.</em></p>
<p>Recall that if <m>z=x+iy</m>, <m>r = |z| = \sqrt{x^{2}+y^{2}}</m> and depending on the quadrant in which your complex number lies, <m>\theta</m> is obtained from <m>\tan^{-1}(y/x)</m>.</p>
<p><span/></p>
<p>In this case, your complex number lies in Quadrant 2 where  <m>\tan^{-1}(y/x) = -{\frac{\pi}{4}}</m>  and <m>\theta = \pi+(-{\frac{\pi}{4}}) = {\frac{3 \pi}{4}}</m>. </p>
<p><span/></p>
<p>So <m>r = {9}</m> and <m>\theta = {\frac{3 \pi}{4}}</m> and hence in  exponential form, <m>z=\displaystyle {9} e^{i({\frac{3 \pi}{4}})}</m>.</p>
<p> </p>
<p>We apply the following formula to get the roots, <m> z_{k}= \displaystyle |z|^{\frac{1}{n}}e^{({\frac{\Theta}{n}}+{\frac{2 \pi k}{n}})i}</m> where <m>n=2</m>, and <m>k=0,1</m>. So,</p>
 
<p><md>
<mrow>z_{k}= \displaystyle {9}^{\frac{1}{2}}e^{({\frac{3 \pi}{8}}+{\pi k})i}</mrow>
</md></p>
 
<p><md>
<mrow>\text{For} \; \amp  k=0, \amp  \displaystyle z_{0}= \displaystyle {3} e^{{\frac{3 \pi}{8}}i}={3} \left( \cos({\frac{3 \pi}{8}}) + i \sin({\frac{3 \pi}{8}}) \right)</mrow>
<mrow>\text{For} \; \amp  k=1, \amp  \displaystyle z_{1}= \displaystyle {3} e^{{-\frac{5 \pi}{8}}i} = {3} \left( \cos({-\frac{5 \pi}{8}}) + i \sin({-\frac{5 \pi}{8}}) \right)</mrow>
</md></p></div></solution>
<answer><p><m>9</m></p></answer>
<answer><p><m>\frac{3 \pi}{4}</m></p></answer>
<answer><p><m>9 e^{\frac{3 \pi}{4} \mathrm{i}}</m></p></answer>
<answer><p><m>9^{\frac{1}{2}} \left(\cos \left( \frac{3 \pi}{8} \right)+\mathrm{i} \sin \left( \frac{3 \pi}{8} \right)\right)</m></p></answer>
<answer><p><m>9^{\frac{1}{2}} \left(\cos \left( -\frac{5 \pi}{8} \right)+\mathrm{i} \sin \left( -\frac{5 \pi}{8} \right)\right)</m></p></answer>
</stack-static>