<stack-static>
<statement><div><p>Write <m>\displaystyle \frac{{27}^{{2}} \cdot {256}^{{4}} \cdot {12}}{{3}^{-{2}} \cdot {4}^{{10}}}</m> in the form <m>{3}^n \cdot {4}^m</m>, where <m>n,m\in \mathbb{Z}</m></p>

<p><fillin characters="15" name="ans1"/>  </p></div></statement>
<solution><div><h3>Worked Solution </h3>

<p>We write out all of the terms in the expression as powers of <m>3</m> and <m>4</m>, and then simplify using the standard laws of incidies.</p>

<p><md number="yes">
<mrow>\displaystyle \frac{{27}^{{2}}\cdot {256}^{{4}}\cdot {12}}{{3}^{-{2}}\cdot {4}^{{10}}} \amp = \displaystyle \frac{({3}^{{3}})^{{2}}\cdot ({4}^{{4}})^{{4}}\cdot {3} \cdot {4}}{{3}^{-{2}}\cdot {4}^{{10}}}</mrow>
<mrow>\amp = \displaystyle \frac{{3}^{{3\cdot 2}}\cdot {4}^{{4\cdot 4}}\cdot {3}^1 \cdot {4}^1}{{3}^{-{2}}\cdot {4}^{{10}}}</mrow>
<mrow>\amp = \displaystyle \frac{{3}^{{6}}\cdot {4}^{{16}}\cdot {3}^1 \cdot {4}^1}{{3}^{-{2}}\cdot {4}^{{10}}}</mrow>
<mrow>\amp = {3}^{{6}+1-(-{2})} \cdot {4}^{{7}}</mrow>
<mrow>\amp = {3}^{{9}} \cdot {4}^{{7}}</mrow>
</md></p></div></solution>
<answer><p><m>3^9\cdot 4^7</m></p></answer>
</stack-static>