<stack-static>
<statement><div><p>If <m>g(x)={2}+{2 x}+e^x</m>, find <m>g^{-1}({3})</m></p>
<p> <m>g^{-1}({3})=</m> <fillin characters="5" name="ans1"/></p></div></statement>
<solution><div><h3>Worked Solution</h3>
<p>In this case we cannot find <m> g^{-1}(x), </m> however we can use some elements of the domain of <m>g</m> to give us the image <m>{3},</m> </p>
<p><m>g(-2)={2}+{2}(-2)+e^{-2}={-2}+\frac{1}{e^{2}}</m></p>
<p><m>g(-1)={2}+{2}(-1)+e^{-1}={0}+\frac{1}{e}</m></p>
<p><m>g(0)={2}+0+e^0={2}+1={3}</m></p>
<p>Thus, <m>g^{-1}({3})=0.</m></p></div></solution>
<answer><p><m>0</m></p></answer>
</stack-static>