<stack-static>
<statement><div><p>Find the center and radius of a circle with <m>A({-5}, {-1})</m> and <m>B({3}, {-1})</m> as endpoints of its diameter.</p>
<p> <alert>Note:</alert> Give your answer in <m>2</m> decimal places where necessary</p>
<p> Centre <m>=</m> <fillin characters="6" name="ans1"/> </p>
<p> Radius <m>=</m> <fillin characters="4" name="ans2"/> units   </p>
<p/>
<p>Note: For the centre coordinates, enter your values inside the parenthesis <m> \left( a, b \right) </m></p></div></statement>
<solution><div><h3>Worked Solution</h3>
<p>Let's apply these steps to the given endpoints <m>A({-5},{-1})</m> and <m>B({3},{-1})</m>:</p>
<p><alert>Step 1:</alert> Find the midpoint (center) of the diameter <m> \displaystyle M= \left(\frac{{x_1 + x_2}}{2}, \frac{{y_1 + y_2}}{2}\right)</m> </p>
<p><md>
<mrow>\text{Midpoint (M)} \amp  =  \left(\frac{{({-5}) + ({3})}}{2}, \frac{{({-1}) + ({-1})}}{2}\right)</mrow>
<mrow>\amp  = \left(\frac{{{-2}}}{2}, \frac{{{-2}}}{2}\right)</mrow>
<mrow>\amp  = \left({-1},{-1} \right)</mrow>
</md></p>
<p><alert>Step 2:</alert> Find the distance (radius) from one of the endpoints to the center. </p>
<p>The distance formula gives us the radius <m>R</m> as:</p>
<me>R = \sqrt{{(x_2 - x_1)^2 + (y_2 - y_1)^2}}</me>
<p>Here we can use the points <m>A({-5},{-1})</m> and center <m> C\left({-1},{-1} \right) </m> to find the radius <m>R</m>. (Note: You can also use <m>B({3},{-1})</m>):
</p>
<p><m> \displaystyle \begin{align}\text{Radius (R)} &amp; =\sqrt{{(({3}) - ({-1}))^2 + (({-1}) - ({-1}))^2}} \\
&amp; = \sqrt{{({4})^2 + ({0})^2}} \\
&amp; = \sqrt{{16}} \\
&amp; = {4}
\end{align} </m></p>
<p>So, the radius of the circle is <m>{4} </m> units</p>
<p>Therefore, the center of the circle is <m> C [{-1},{-1} ] </m> and the radius is <m>{4}</m> units.</p></div></solution>
<answer><p><m>\left[ -1 , -1 \right] </m></p></answer>
<answer><p><m>4</m></p></answer>
</stack-static>